better modeling of automatagitk

PDS/PDS.thy
@@ -12,17 +12,9 @@ text \<open>We define push down systems.\<close>
 
 locale PDS =
   (* 'ctr_loc is the type of control locations *)
-  fixes P_locs :: "'ctr_loc::finite set" 
-    and \<Delta> :: "('ctr_loc, 'label::finite) rule set"
-    (*    and c0 :: "('ctr_loc, 'label) conf" *)
-  assumes \<Delta>_subset: "\<Delta> \<subseteq> (P_locs \<times> UNIV) \<times> (P_locs \<times> UNIV)"
+  fixes \<Delta> :: "('ctr_loc, 'label::finite) rule set"
+  
 begin
-
-lemma finite_P_locs: "finite P_locs"
-  by simp
-
-fun config_wf :: "('ctr_loc, 'label) conf \<Rightarrow> bool" where
-  "config_wf (c, l) \<longleftrightarrow> c \<in> P_locs"
 
 primrec op_labels :: "'label operation \<Rightarrow> 'label list" where
   "op_labels pop = []"
@@ -42,29 +34,7 @@ notation step_starp (infix "\<Rightarrow>\<^sup>*" 80)
 
 lemma step_relp_def2:
   "(p, \<gamma>w') \<Rightarrow> (p',ww') \<longleftrightarrow> (\<exists>\<gamma> w' w. \<gamma>w' = \<gamma>#w' \<and> ww' = (op_labels w)@w' \<and> (p, \<gamma>) \<hookrightarrow> (p', w))"
-  by (metis (no_types, lifting) PDS.transition_rel.intros PDS_axioms step_relp_def transition_rel.cases)
-
-lemma step_relp'_P_locs1:
-  assumes "(q1, x) \<Rightarrow> (q2, y)"
-  shows "q1 \<in> P_locs"
-proof -
-  from assms have "\<exists>\<gamma> w. (q1, \<gamma>) \<hookrightarrow> (q2, w)"
-    by (metis PDS.transition_rel.cases PDS_axioms step_relp_def)
-  then show "?thesis"
-    using \<Delta>_subset unfolding is_rule_def
-    by auto
-qed
-
-lemma step_relp'_P_locs2:
-  assumes "(q1, x) \<Rightarrow> (q2, y)"
-  shows "q2 \<in> P_locs"
-proof -
-  from assms have "\<exists>\<gamma> w. (q1, \<gamma>) \<hookrightarrow> (q2, w)"
-    by (metis PDS.transition_rel.cases PDS_axioms step_relp_def)
-  then show "?thesis"
-    using \<Delta>_subset unfolding is_rule_def
-    by auto
-qed
+  by (metis (no_types, lifting) PDS.transition_rel.intros step_relp_def transition_rel.cases)
 
 end
 
@@ -73,70 +43,89 @@ section \<open>PDS with P automaton\<close>
 
 type_synonym ('ctr_loc, 'label) sat_rule = "('ctr_loc, 'label) transition set \<Rightarrow> ('ctr_loc, 'label) transition set \<Rightarrow> bool"
 
-datatype ('ctr_loc, 'label) ctr_loc =
-  is_Ctr_Loc: Ctr_Loc (the_Ctr_Loc: 'ctr_loc)
-  | is_Ctr_Ext: Ctr_Loc_Ext (the_Ext_Ctr_Loc: 'ctr_loc) (the_Ext_Label: 'label)
+datatype ('ctr_loc, 'state, 'label) state =
+  is_Ctr_Loc: Ctr_Loc (the_Ctr_Loc: 'ctr_loc) (* p \<in> P *)
+  | is_State: Ctr_Loc_St (the_St: 'state) (* q \<in> Q \<and> q \<notin> P *)
+  | is_Ctr_Ext: Ctr_Loc_Ext (the_Ext_Ctr_Loc: 'ctr_loc) (the_Ext_Label: 'label) (* q\<^sub>p\<^sub>\<gamma> *)
+
 
 find_theorems "finite UNIV"
 find_theorems class.finite
 
 lemma finite_ctr_locs:
   assumes "finite (UNIV :: 'ctr_loc set)"
+  assumes "finite (UNIV :: 'state set)"
   assumes "finite (UNIV :: 'label set)"
-  shows "finite (UNIV :: ('ctr_loc, 'label) ctr_loc set)"
+  shows "finite (UNIV :: ('ctr_loc, 'state, 'label) state set)"
 proof -
-  define Ctr_Loc_Ext' where "Ctr_Loc_Ext' == \<lambda>(c :: 'ctr_loc, l:: 'label). Ctr_Loc_Ext c l"
+  define Ctr_Loc_Ext' :: "('ctr_loc * 'label) \<Rightarrow> ('ctr_loc, 'state, 'label) state" where 
+    "Ctr_Loc_Ext' == \<lambda>(c :: 'ctr_loc, l:: 'label). Ctr_Loc_Ext c l"
+  define Ctr_Loc' :: "'ctr_loc \<Rightarrow> ('ctr_loc, 'state, 'label) state" where
+    "Ctr_Loc' = Ctr_Loc"
+  define Ctr_Loc_St' :: "'state \<Rightarrow> ('ctr_loc, 'state, 'label) state" where
+    "Ctr_Loc_St' = Ctr_Loc_St"
 
-  have "finite (Ctr_Loc ` (UNIV:: 'ctr_loc set))"
+  have split: "UNIV = (Ctr_Loc' ` UNIV) \<union> (Ctr_Loc_St' ` UNIV) \<union> (Ctr_Loc_Ext' ` (UNIV :: (('ctr_loc * 'label) set)))"
+    unfolding Ctr_Loc'_def Ctr_Loc_St'_def
+  proof (rule; rule; rule; rule)
+    fix x :: "('ctr_loc, 'state, 'label) state"
+    assume "x \<in> UNIV"
+    moreover
+    assume "x \<notin> range Ctr_Loc_Ext'"
+    moreover
+    assume "x \<notin> range Ctr_Loc_St"
+    ultimately
+    show "x \<in> range Ctr_Loc"
+      by (metis Ctr_Loc_Ext'_def prod.simps(2) range_eqI state.exhaust)
+  qed
+
+  have "finite (Ctr_Loc' ` (UNIV:: 'ctr_loc set))"
+    using assms by auto
+  moreover
+  have "finite (Ctr_Loc_St' ` (UNIV:: 'state set))"
     using assms by auto
   moreover
   have "finite (UNIV :: (('ctr_loc * 'label) set))"
     using assms by (simp add: finite_Prod_UNIV)
-  then have b: "finite (Ctr_Loc_Ext' ` (UNIV :: (('ctr_loc * 'label) set)))"
+  then have "finite (Ctr_Loc_Ext' ` (UNIV :: (('ctr_loc * 'label) set)))"
     by auto
-  moreover
-  have c: "UNIV = (Ctr_Loc ` UNIV) \<union> (Ctr_Loc_Ext' ` (UNIV :: (('ctr_loc * 'label) set)))"
-    unfolding Ctr_Loc_Ext'_def using UNIV_I UnCI ctr_loc.exhaust equalityI image_eqI split_conv subsetI by smt
   ultimately
-  show ?thesis
-    unfolding c by auto
+  show "finite (UNIV :: ('ctr_loc, 'state, 'label) state set)"
+    unfolding split by auto
 qed
 
-instantiation ctr_loc :: (finite, finite) finite begin
-
-(* Man kunne vise at der ikke er en injection
-   fra nat til vores type. *)
+instantiation state :: (finite, finite, finite) finite begin
 
 instance by standard (simp add: finite_ctr_locs)
 
 end
 
 
-locale PDS_with_P_automaton = PDS P_locs \<Delta>
-  for P_locs :: "'ctr_loc::finite set" and \<Delta> :: "('ctr_loc, 'label::finite) rule set"
+locale PDS_with_P_automaton = PDS \<Delta>
+  for \<Delta> :: "('ctr_loc::finite, 'label::finite) rule set"
     +
-  fixes Q_locs :: "'ctr_loc set" (* I think we should just see Q as the whole type. So this can be deleted *)
-    (*    and trans :: "('ctr_loc, 'label) transition set" *)
-    and F_locs :: "'ctr_loc set"
-  assumes "P_locs \<subseteq> Q_locs"
-    (*    and "trans \<subseteq> Q_locs \<times> UNIV \<times> Q_locs" *)
-    and "F_locs \<subseteq> Q_locs"
+  fixes F_locs :: "('ctr_loc, 'state::finite, 'label) state set"
+  assumes "\<not>(\<exists>f\<in>F_locs. is_Ctr_Ext f)"
 begin
+
+definition P_locs :: "('ctr_loc, 'state, 'label) state set" where 
+  "P_locs = {q. is_Ctr_Loc q}"
+
+definition Old_Aut_states :: "('ctr_loc, 'state, 'label) state set" where
+  "Old_Aut_states = {q. is_State q}"
+
+definition New_Aut_states :: "('ctr_loc, 'state, 'label) state set" where
+  "New_Aut_states = {q. is_Ctr_Ext q}"
 
 interpretation LTS transition_rel .
 notation step_relp (infix "\<Rightarrow>" 80)
 notation step_starp (infix "\<Rightarrow>\<^sup>*" 80)
 
+definition accepts :: "(('ctr_loc, 'state, 'label) state, 'label) transition set \<Rightarrow> ('ctr_loc , 'label) conf \<Rightarrow> bool" where
+  "accepts ts \<equiv> \<lambda>(p,w). (\<exists>q \<in> F_locs. (Ctr_Loc p,w,q) \<in> LTS.transition_star ts)"
 
-term "(q,w) :: ('ctr_loc , 'label) conf"
-
-
-definition accepts :: "('ctr_loc, 'label) transition set \<Rightarrow> ('ctr_loc , 'label) conf \<Rightarrow> bool" where
-  "accepts ts \<equiv> \<lambda>(p,w). (\<exists>q \<in> F_locs. (p,w,q) \<in> LTS.transition_star ts)"
-  (* Here acceptance is defined for any p, but in the paper p has to be in P_locs. FIX this!!!!!!!! *)
-
-definition accepts_\<epsilon> :: "(('ctr_loc, 'label) ctr_loc, 'label option) transition set \<Rightarrow> (('ctr_loc, 'label) ctr_loc, 'label) conf \<Rightarrow> bool" where
-  "accepts_\<epsilon> ts \<equiv> \<lambda>(p,w). (\<exists>q \<in> F_locs. (p,w,Ctr_Loc q) \<in> LTS_\<epsilon>.transition_star_\<epsilon> ts)"
+definition accepts_\<epsilon> :: "(('ctr_loc, 'state, 'label) state, 'label option) transition set \<Rightarrow> ('ctr_loc, 'label) conf \<Rightarrow> bool" where
+  "accepts_\<epsilon> ts \<equiv> \<lambda>(p,w). (\<exists>q \<in> F_locs. (Ctr_Loc p,w,q) \<in> LTS_\<epsilon>.transition_star_\<epsilon> ts)"
 
 abbreviation \<epsilon> :: "'label option" where
   "\<epsilon> == None"
@@ -144,14 +133,14 @@ abbreviation \<epsilon> :: "'label option" where
 lemma accepts_mono[mono]: "mono accepts" (* Hmm.. what does this actually mean? *)
 proof (rule, rule)
   fix c :: "('ctr_loc, 'label) conf"
-  fix ts ts' :: "('ctr_loc, 'label) transition set"
+  fix ts ts' :: "(('ctr_loc, 'state, 'label) state, 'label) transition set"
   assume accepts_xa: "accepts ts c"
   assume tsts': "ts \<subseteq> ts'"
   obtain p l where pl_p: "c = (p,l)"
     by (cases c)
-  obtain q where q_p:  "q \<in> F_locs \<and> (p, l, q) \<in> LTS.transition_star ts"
+  obtain q where q_p:  "q \<in> F_locs \<and> (Ctr_Loc p, l, q) \<in> LTS.transition_star ts"
     using accepts_xa unfolding pl_p accepts_def by auto
-  then have "(p, l, q) \<in> LTS.transition_star ts'"
+  then have "(Ctr_Loc p, l, q) \<in> LTS.transition_star ts'"
     using tsts' LTS_transition_star_mono monoD by blast 
   then have "accepts ts' (p,l)"
     unfolding accepts_def using q_p by auto
@@ -159,36 +148,13 @@ proof (rule, rule)
     unfolding pl_p .
 qed
 
-lemma accepts_cons: "(p, \<gamma>, q) \<in> ts \<Longrightarrow> accepts ts (q, w) \<Longrightarrow> accepts ts (p, \<gamma> # w)"
-  using LTS.transition_star.transition_star_step accepts_def PDS_with_P_automaton_axioms by fastforce
+lemma accepts_cons: "(Ctr_Loc p, \<gamma>, Ctr_Loc p') \<in> ts \<Longrightarrow> accepts ts (p', w) \<Longrightarrow> accepts ts (p, \<gamma> # w)"
+  using LTS.transition_star.transition_star_step accepts_def by fastforce 
 
-lemma accepts_unfold: "accepts ts (p, \<gamma> # w) \<Longrightarrow> \<exists>q. (p, \<gamma>, q) \<in> ts \<and> accepts ts (q, w)"
-  using LTS.transition_star_cons accepts_def case_prod_conv by force 
-
-lemma accepts_unfoldn: "accepts ts (p, w' @ w) \<Longrightarrow> \<exists>q. (p, w', q) \<in> LTS.transition_star ts \<and> accepts ts (q, w)"
-proof (induct w' arbitrary: p w)
-  case Nil
-  then show ?case by (metis LTS.transition_star.transition_star_refl append_Nil)
-next
-  case (Cons a w')
-  then show ?case by (metis LTS.transition_star.transition_star_step accepts_unfold append_Cons)
-qed
-
-lemma accepts_append: "(p, w', q) \<in> LTS.transition_star ts \<Longrightarrow> accepts ts (q, w) \<Longrightarrow> accepts ts (p, w' @ w)"
-proof (induct w' arbitrary: w p q)
-  case Nil
-  then show ?case 
-    by (metis LTS.transition_star_empty append_Nil)
-next
-  case (Cons a w')
-  then show ?case 
-    by (metis LTS.transition_star_cons accepts_cons append_Cons)
-qed
-
-definition language :: "('ctr_loc, 'label) transition set \<Rightarrow> ('ctr_loc, 'label) conf set" where
+definition language :: "(('ctr_loc, 'state, 'label) state, 'label) transition set \<Rightarrow> ('ctr_loc, 'label) conf set" where
   "language ts = {c. accepts ts c}"
 
-definition language_\<epsilon> :: "(_, 'label option) transition set \<Rightarrow> (_, 'label) conf set" where
+definition language_\<epsilon> :: "(('ctr_loc, 'state, 'label) state, 'label option) transition set \<Rightarrow> ('ctr_loc, 'label) conf set" where
   "language_\<epsilon> ts = {c. accepts_\<epsilon> ts c}"
 
 
@@ -203,11 +169,11 @@ definition saturation :: "('c, 'l) sat_rule \<Rightarrow> ('c, 'l) transition se
 
 subsection \<open>Saturation rules\<close>
 
-inductive pre_star_rule :: "('ctr_loc, 'label) transition set \<Rightarrow> ('ctr_loc, 'label) transition set \<Rightarrow> bool" where (* TODO: p' should also be in P_locs I guess... *)
-  add_trans: "(p, \<gamma>) \<hookrightarrow> (p', w) \<Longrightarrow> p \<in> P_locs \<Longrightarrow> (p', op_labels w, q) \<in> LTS.transition_star ts \<Longrightarrow> (p, \<gamma>, q) \<notin> ts \<Longrightarrow> pre_star_rule ts (ts \<union> {(p, \<gamma>, q)})"
+inductive pre_star_rule :: "(('ctr_loc, 'state, 'label) state, 'label) transition set \<Rightarrow> (('ctr_loc, 'state, 'label) state, 'label) transition set \<Rightarrow> bool" where 
+  add_trans: "(p, \<gamma>) \<hookrightarrow> (p', w) \<Longrightarrow> (Ctr_Loc p', op_labels w, q) \<in> LTS.transition_star ts \<Longrightarrow> (Ctr_Loc p, \<gamma>, q) \<notin> ts \<Longrightarrow> pre_star_rule ts (ts \<union> {(Ctr_Loc p, \<gamma>, q)})"
 
-inductive post_star_rules :: "(('ctr_loc, 'label) ctr_loc, 'label option) transition set \<Rightarrow> (('ctr_loc, 'label) ctr_loc, 'label option) transition set \<Rightarrow> bool" where
-  add_trans_pop: "(p, \<gamma>) \<hookrightarrow> (p', pop) \<Longrightarrow> p' \<in> P_locs \<Longrightarrow> (Ctr_Loc p, [\<gamma>], q) \<in> LTS_\<epsilon>.transition_star_\<epsilon> ts \<Longrightarrow> (Ctr_Loc p', \<epsilon>, q) \<notin> ts \<Longrightarrow> post_star_rules ts (ts \<union> {(Ctr_Loc p', \<epsilon>, q)})"
+inductive post_star_rules :: "(('ctr_loc, 'state, 'label) state, 'label option) transition set \<Rightarrow> (('ctr_loc, 'state, 'label) state, 'label option) transition set \<Rightarrow> bool" where
+  add_trans_pop: "(p, \<gamma>) \<hookrightarrow> (p', pop) \<Longrightarrow> (Ctr_Loc p, [\<gamma>], q) \<in> LTS_\<epsilon>.transition_star_\<epsilon> ts \<Longrightarrow> (Ctr_Loc p', \<epsilon>, q) \<notin> ts \<Longrightarrow> post_star_rules ts (ts \<union> {(Ctr_Loc p', \<epsilon>, q)})"
 | add_trans_swap: "(p, \<gamma>) \<hookrightarrow> (p', swap \<gamma>') \<Longrightarrow> (Ctr_Loc p, [\<gamma>], q) \<in> LTS_\<epsilon>.transition_star_\<epsilon> ts \<Longrightarrow> (Ctr_Loc p', Some \<gamma>', q) \<notin> ts \<Longrightarrow> post_star_rules ts (ts \<union> {(Ctr_Loc p', Some \<gamma>', q)})"
 | add_trans_push_1: "(p, \<gamma>) \<hookrightarrow> (p', push \<gamma>' \<gamma>'') \<Longrightarrow> (Ctr_Loc p, [\<gamma>], q) \<in> LTS_\<epsilon>.transition_star_\<epsilon> ts \<Longrightarrow> (Ctr_Loc p', Some \<gamma>', Ctr_Loc_Ext p' \<gamma>') \<notin> ts \<Longrightarrow> post_star_rules ts (ts \<union> {(Ctr_Loc p', Some \<gamma>', Ctr_Loc_Ext p' \<gamma>')})"
 | add_trans_push_2: "(p, \<gamma>) \<hookrightarrow> (p', push \<gamma>' \<gamma>'') \<Longrightarrow> (Ctr_Loc p, [\<gamma>], q) \<in> LTS_\<epsilon>.transition_star_\<epsilon> ts \<Longrightarrow> (Ctr_Loc_Ext p' \<gamma>', Some \<gamma>'', q) \<notin> ts \<Longrightarrow> (Ctr_Loc p', Some \<gamma>', Ctr_Loc_Ext p' \<gamma>') \<in> ts \<Longrightarrow> post_star_rules ts (ts \<union> {(Ctr_Loc_Ext p' \<gamma>', Some \<gamma>'', q)})"
@@ -430,7 +396,7 @@ lemma  lemma_3_1:
   using assms
 proof (induct rule: converse_rtranclp_induct)
   case base
-  then have "\<exists>q \<in> F_locs. (fst pv, snd pv, q) \<in> LTS.transition_star A'"
+  then have "\<exists>q \<in> F_locs. (Ctr_Loc (fst pv), snd pv, q) \<in> LTS.transition_star A'"
     unfolding language_def using pre_star_lim'_incr_transition_star accepts_def by fastforce 
   then show ?case
     unfolding accepts_def by auto
@@ -447,55 +413,53 @@ next
 
   then have "accepts A' (p'', u)" 
     using step unfolding p''u_def by auto
-  then obtain q where q_p: "q \<in> F_locs \<and> (p'', u, q) \<in> LTS.transition_star A'"
+  then obtain q where q_p: "q \<in> F_locs \<and> (Ctr_Loc p'', u, q) \<in> LTS.transition_star A'"
     unfolding accepts_def using p''_def u_def by auto
   have "\<exists>\<gamma> w1 u1. w=\<gamma>#w1 \<and> u=op_labels u1@w1 \<and> (p', \<gamma>) \<hookrightarrow> (p'', u1)"
     using p''u_def p'w_def step.hyps(1) step_relp_def2 by auto
   then obtain \<gamma> w1 u1 where \<gamma>_w1_u1_p: "w=\<gamma>#w1 \<and> u=op_labels u1@w1 \<and> (p', \<gamma>) \<hookrightarrow> (p'', u1)"
     by blast
 
-  have p'_P_locs: "p' \<in> P_locs"
-    using p''u_def p'w_def step.hyps(1) step_relp'_P_locs1 by auto
-
-  have "\<exists>q1. (p'', op_labels u1, q1) \<in> LTS.transition_star A' \<and> (q1, w1, q) \<in> LTS.transition_star A'"
+  have "\<exists>q1. (Ctr_Loc p'', op_labels u1, q1) \<in> LTS.transition_star A' \<and> (q1, w1, q) \<in> LTS.transition_star A'"
     using q_p \<gamma>_w1_u1_p LTS.transition_star_split by auto
 
-  then obtain q1 where q1_p: "(p'', op_labels u1, q1) \<in> LTS.transition_star A' \<and> (q1, w1, q) \<in> LTS.transition_star A'"
+  then obtain q1 where q1_p: "(Ctr_Loc p'', op_labels u1, q1) \<in> LTS.transition_star A' \<and> (q1, w1, q) \<in> LTS.transition_star A'"
     by auto
 
-  then have in_A': "(p', \<gamma>, q1) \<in> A'"
+  then have in_A': "(Ctr_Loc p', \<gamma>, q1) \<in> A'"
     using \<gamma>_w1_u1_p 
     using add_trans[of p' \<gamma> p'' u1 q1 A'] 
     using step.prems(2)
     using saturated_def
     using saturation_def[of ]
     using step.prems
-    using p'_P_locs
     by metis
 
-  then have "(p', \<gamma>#w1, q) \<in> LTS.transition_star A'"
+  then have "(Ctr_Loc p', \<gamma>#w1, q) \<in> LTS.transition_star A'"
     using in_A' transition_star_step q1_p
     by (meson LTS.transition_star.transition_star_step)
-  then have t_in_A': "(p', w, q) \<in> LTS.transition_star A'"
+  then have t_in_A': "(Ctr_Loc p', w, q) \<in> LTS.transition_star A'"
     using \<gamma>_w1_u1_p by blast
 
-  from q_p t_in_A' have "q \<in> F_locs \<and> (p', w, q) \<in> LTS.transition_star A'"
+  from q_p t_in_A' have "q \<in> F_locs \<and> (Ctr_Loc p', w, q) \<in> LTS.transition_star A'"
     using p'_def w_def by auto
   then show ?case
     unfolding accepts_def p'w_def using q_p by auto 
 qed
 
 lemma lemma_3_2_base: 
-  "(p, w, q) \<in> LTS.transition_star rel \<Longrightarrow> \<exists>p' w'. (p, w) \<Rightarrow>\<^sup>* (p', w') \<and> (p', w', q) \<in> LTS.transition_star rel"
+  "(Ctr_Loc p, w, q) \<in> LTS.transition_star rel \<Longrightarrow> \<exists>p' w'. (p, w) \<Rightarrow>\<^sup>* (p', w') \<and> (Ctr_Loc p', w',  q) \<in> LTS.transition_star rel"
   by auto
 
 lemma pre_star_rule_mono': "t \<in> LTS.transition_star rel \<Longrightarrow> pre_star_rule rel rel' \<Longrightarrow> t \<in> LTS.transition_star (rel')"
   using pre_star'_incr_transition_star by blast
 
-lemma lemma_3_2_b_aux:
+
+
+lemma lemma_3_2_b_aux':
   (* Lemma from discussion with Morten 2 *)
   assumes "(p, w, ss, q) \<in> LTS.transition_star_states A"
-  assumes "\<nexists>q \<gamma> q'. (q, \<gamma>, q') \<in> A \<and> q' \<in> P_locs"
+  assumes "\<nexists>q \<gamma> q'. (q, \<gamma>, Ctr_Loc q') \<in> A"
   assumes "q \<in> P_locs"
   shows "w = [] \<and> p = q \<and> ss=[p]"
   using assms 
@@ -504,10 +468,29 @@ proof(induction rule: LTS.transition_star_states.induct[OF assms(1)])
   then show ?case by auto
 next
   case (2 p \<gamma> q' w ss q)
-  then show ?case by auto
+  then show ?case
+    by (metis P_locs_def is_Ctr_Loc_def mem_Collect_eq)
 qed
 
-lemma lemma_3_2_b:
+lemma lemma_3_2_b_aux:
+  (* Lemma from discussion with Morten 2 *)
+  fixes A :: "(('ctr_loc, 'state, 'label) state, 'label) transition set"
+  assumes "(p, w, ss, Ctr_Loc q) \<in> LTS.transition_star_states A"
+  assumes "\<nexists>q \<gamma> q'. (q, \<gamma>, Ctr_Loc q') \<in> A"
+  shows "w = [] \<and> p = Ctr_Loc q \<and> ss=[p]"
+proof -
+  have "Ctr_Loc q \<in> P_locs"
+    unfolding P_locs_def by auto
+  moreover
+  have "\<nexists>q \<gamma> q'. (q, \<gamma>, q') \<in> A \<and> q' \<in> P_locs"
+    using assms(2) unfolding P_locs_def by (metis is_Ctr_Loc_def mem_Collect_eq) 
+  ultimately 
+  show ?thesis
+    using lemma_3_2_b_aux' assms(1) assms(2) by blast
+qed
+
+
+lemma lemma_3_2_b':
   (* The natural langauge formulation of this in the thesis is quite strange. *)
   assumes "(p, w, q) \<in> LTS.transition_star A"
   assumes "\<nexists>q \<gamma> q'. (q, \<gamma>, q') \<in> A \<and> q' \<in> P_locs"
@@ -522,7 +505,22 @@ next
   then show ?case by blast
 qed
 
-
+lemma lemma_3_2_b:
+  (* The natural langauge formulation of this in the thesis is quite strange. *)
+  fixes A :: "(('ctr_loc, 'state, 'label) state, 'label) transition set"
+  assumes "(p, w, Ctr_Loc q) \<in> LTS.transition_star A"
+  assumes "\<nexists>q \<gamma> q'. (q, \<gamma>, Ctr_Loc q') \<in> A"
+  shows "w = [] \<and> p = Ctr_Loc q"
+proof -
+  have "Ctr_Loc q \<in> P_locs"
+    unfolding P_locs_def by auto
+  moreover
+  have "\<nexists>q \<gamma> q'. (q, \<gamma>, q') \<in> A \<and> q' \<in> P_locs"
+    using assms(2) unfolding P_locs_def by (metis is_Ctr_Loc_def mem_Collect_eq) 
+  ultimately 
+  show ?thesis
+    using lemma_3_2_b' assms(1) by blast
+qed
 
 lemma step_relp_append_aux:
   assumes "pu \<Rightarrow>\<^sup>* p1y"
@@ -553,7 +551,7 @@ next
   then obtain \<gamma> w' wa where \<gamma>_w'_wa_p: " w = \<gamma> # w' \<and> y = op_labels wa @ w' \<and> (p', \<gamma>) \<hookrightarrow> (p1, wa)"
     by metis
   then have "(p, u @ v) \<Rightarrow>\<^sup>* (p1, y @ v)"
-    by (metis (no_types, lifting) PDS.step_relp_def2 PDS_axioms append.assoc append_Cons rtranclp.simps step_3)
+    by (metis (no_types, lifting) PDS.step_relp_def2 append.assoc append_Cons rtranclp.simps step_3)
   then show ?case
     by (simp add: p1_def p_def u_def y_def)
 qed
@@ -569,10 +567,10 @@ lemma step_relp_append_empty:
   using step_relp_append[OF assms] by auto  
 
 lemma lemma_3_2_a':
-  assumes "\<nexists>q \<gamma> q'. (q, \<gamma>, q') \<in> A \<and> q' \<in> P_locs"
+  assumes "\<nexists>q \<gamma> q'. (q, \<gamma>, Ctr_Loc q') \<in> A"
   assumes "pre_star_rule\<^sup>*\<^sup>* A A'"
-  assumes "(p, w, ss, q) \<in> LTS.transition_star_states A'"
-  shows "\<exists>p' w' ss'. (p', w', ss', q) \<in> LTS.transition_star_states A \<and> (p, w) \<Rightarrow>\<^sup>* (p', w')"
+  assumes "(Ctr_Loc p, w, ss, q) \<in> LTS.transition_star_states A'"
+  shows "\<exists>p' w' ss'. (Ctr_Loc p', w', ss', q) \<in> LTS.transition_star_states A \<and> (p, w) \<Rightarrow>\<^sup>* (p', w')"
   using assms(2) assms(1,3) 
 proof (induction arbitrary: p q w ss rule: rtranclp_induct)
   case base
@@ -582,78 +580,81 @@ next
   case (step Aiminus1 Ai)
 
   from step(2) obtain p1 \<gamma> p2 w2 q' where p1_\<gamma>_p2_w2_q'_p:
-    "Ai = Aiminus1 \<union> {(p1, \<gamma>, q')}" 
+    "Ai = Aiminus1 \<union> {(Ctr_Loc p1, \<gamma>, q')}" 
     "(p1, \<gamma>) \<hookrightarrow> (p2, w2)"
-    "(p2, op_labels w2, q') \<in> LTS.transition_star Aiminus1"
-    "(p1, \<gamma>, q') \<notin> Aiminus1"
-    "p1 \<in> P_locs"
+    "(Ctr_Loc p2, op_labels w2, q') \<in> LTS.transition_star Aiminus1"
+    "(Ctr_Loc p1, \<gamma>, q') \<notin> Aiminus1"
     by (meson pre_star_rule.cases)
+
+  have "Ctr_Loc p1 \<in> P_locs"
+    unfolding P_locs_def by auto
 
   note ss_p = step(5)
 
-  define t where "t = (p1, \<gamma>, q')"
-  define j where "j = count (transitions_of' (p, w, ss, q)) t"
+  define t :: "(('ctr_loc, 'state, 'label) state, 'label) transition"
+    where "t = (Ctr_Loc p1, \<gamma>, q')"
+  define j where "j = count (transitions_of' (Ctr_Loc p, w, ss, q)) t"
 
   from j_def ss_p show ?case
   proof (induction j arbitrary: p q w ss)
     case 0
-    have "(p, w, ss, q) \<in> LTS.transition_star_states Aiminus1"
+    have "(Ctr_Loc p, w, ss, q) \<in> LTS.transition_star_states Aiminus1"
       using lemma_3_2_a'_Aux_3
         p1_\<gamma>_p2_w2_q'_p(1) t_def 0 by fastforce
     then show ?case
       using step.IH step.prems(1) by metis
   next
     case (Suc j')
-    have "\<exists>u v u_ss v_ss. ss = u_ss@v_ss \<and> w = u@[\<gamma>]@v \<and> (p,u,u_ss,p1) \<in> LTS.transition_star_states Aiminus1 \<and> (p1,[\<gamma>],q') \<in> LTS.transition_star Ai \<and> (q',v,v_ss,q) \<in> LTS.transition_star_states Ai"
-      apply (rule split_at_first_t[of p w ss q Ai j' p1 \<gamma> q' Aiminus1])
+    have "\<exists>u v u_ss v_ss. ss = u_ss@v_ss \<and> w = u@[\<gamma>]@v \<and> (Ctr_Loc p,u,u_ss, Ctr_Loc p1) \<in> LTS.transition_star_states Aiminus1 \<and> (Ctr_Loc p1,[\<gamma>],q') \<in> LTS.transition_star Ai \<and> (q',v,v_ss,q) \<in> LTS.transition_star_states Ai"
+      apply (rule split_at_first_t[of "Ctr_Loc p" w ss q Ai j' "Ctr_Loc p1" \<gamma> q' Aiminus1])
       using Suc(2,3) t_def  p1_\<gamma>_p2_w2_q'_p(1,4) t_def by auto
     then obtain u v u_ss v_ss where u_v_u_ss_v_ss_p:
       "ss = u_ss@v_ss \<and> w = u@[\<gamma>]@v" 
-      "(p,u,u_ss,p1) \<in> LTS.transition_star_states Aiminus1" 
-      "(p1,[\<gamma>],q') \<in> LTS.transition_star Ai" 
+      "(Ctr_Loc p,u,u_ss, Ctr_Loc p1) \<in> LTS.transition_star_states Aiminus1" 
+      "(Ctr_Loc p1,[\<gamma>],q') \<in> LTS.transition_star Ai" 
       "(q',v,v_ss,q) \<in> LTS.transition_star_states Ai"
       by blast
-    have II: "p1 \<in> P_locs"
-      using p1_\<gamma>_p2_w2_q'_p by auto
-    have "\<exists>p'' w'' ss''. (p'', w'', ss'', p1) \<in> LTS.transition_star_states A \<and> (p, u) \<Rightarrow>\<^sup>* (p'', w'')"
-      using Suc(1)[of p u _ p1]
-      using \<open>(p, u, u_ss, p1) \<in> LTS.transition_star_states Aiminus1\<close> step.IH step.prems(1) by blast 
-    then obtain p'' w'' ss'' where "(p'', w'', ss'', p1) \<in> LTS.transition_star_states A" "(p, u) \<Rightarrow>\<^sup>* (p'', w'')"
+    have II: "Ctr_Loc p1 \<in> P_locs"
+      unfolding P_locs_def by auto
+    have "\<exists>p'' w'' ss''. (Ctr_Loc p'', w'', ss'', Ctr_Loc p1) \<in> LTS.transition_star_states A \<and> (p, u) \<Rightarrow>\<^sup>* (p'', w'')"
+      using Suc(1)[of p u _ "Ctr_Loc p1"]
+      using \<open>(Ctr_Loc p, u, u_ss, Ctr_Loc p1) \<in> LTS.transition_star_states Aiminus1\<close> step.IH step.prems(1) by blast 
+    then obtain p'' w'' ss'' where "(Ctr_Loc p'', w'', ss'', Ctr_Loc p1) \<in> LTS.transition_star_states A" "(p, u) \<Rightarrow>\<^sup>* (p'', w'')"
       by blast
-    from this lemma_3_2_b_aux  this(1) II have VIII: "(p, u) \<Rightarrow>\<^sup>* (p1, [])"
-      using step.prems(1) by metis
+    from this this(1) II have VIII: "(p, u) \<Rightarrow>\<^sup>* (p1, [])"
+      using step.prems(1) lemma_3_2_b_aux' by blast 
 
     note IX = p1_\<gamma>_p2_w2_q'_p(2)
     note III = p1_\<gamma>_p2_w2_q'_p(3)
-    from III have III_2: "\<exists>w2_ss. (p2, op_labels w2, w2_ss, q') \<in> LTS.transition_star_states Aiminus1"
-      using LTS.transition_star_transition_star_states[of p2 "op_labels w2" q' Aiminus1] by auto
-    then obtain w2_ss where III_2: "(p2, op_labels w2, w2_ss, q') \<in> LTS.transition_star_states Aiminus1"
+    from III have III_2: "\<exists>w2_ss. (Ctr_Loc p2, op_labels w2, w2_ss, q') \<in> LTS.transition_star_states Aiminus1"
+      using LTS.transition_star_transition_star_states[of "Ctr_Loc p2" "op_labels w2" q' Aiminus1] by auto
+    then obtain w2_ss where III_2: "(Ctr_Loc p2, op_labels w2, w2_ss, q') \<in> LTS.transition_star_states Aiminus1"
       by blast
 
-    from III have V: "(p2, op_labels w2, w2_ss, q') \<in> LTS.transition_star_states Aiminus1" "(q', v, v_ss, q) \<in> LTS.transition_star_states Ai"
+    from III have V: "(Ctr_Loc p2, op_labels w2, w2_ss, q') \<in> LTS.transition_star_states Aiminus1" "(q', v, v_ss, q) \<in> LTS.transition_star_states Ai"
       using III_2 \<open>(q', v, v_ss, q) \<in> LTS.transition_star_states Ai\<close> by auto
 
     define w2v where "w2v = op_labels w2 @ v"
     define w2v_ss where "w2v_ss = w2_ss @ tl v_ss"
 
-    from V(1) have "(p2, op_labels w2, w2_ss, q') \<in> LTS.transition_star_states Ai"
-      using transition_star_states_mono p1_\<gamma>_p2_w2_q'_p(1) by (metis Un_iff subsetI) 
-    then have V_merged: "(p2, w2v, w2v_ss, q) \<in> LTS.transition_star_states Ai"
+    from V(1) have "(Ctr_Loc p2, op_labels w2, w2_ss, q') \<in> LTS.transition_star_states Ai"
+      using transition_star_states_mono p1_\<gamma>_p2_w2_q'_p(1) using Un_iff subsetI by (metis (no_types, hide_lams))
+    then have V_merged: "(Ctr_Loc p2, w2v, w2v_ss, q) \<in> LTS.transition_star_states Ai"
       using V(2) unfolding w2v_def w2v_ss_def by (meson LTS.transition_star_states_append)
 
-    have j'_count: "j' = count (transitions_of' (p2, w2v, w2v_ss, q)) t"
+    have j'_count: "j' = count (transitions_of' (Ctr_Loc p2, w2v, w2v_ss, q)) t"
     proof -
-      have "Suc j' = count (transitions_of' (p, u, u_ss, p1)) t + 1 + count (transitions_of' (q', v, v_ss, q)) t"
+      have "Suc j' = count (transitions_of' (Ctr_Loc p, u, u_ss, Ctr_Loc p1)) t + 1 + count (transitions_of' (q', v, v_ss, q)) t"
         using u_v_u_ss_v_ss_p(2) u_v_u_ss_v_ss_p(4)
         using count_combine_transition_star_states Suc(2) u_v_u_ss_v_ss_p(1) t_def by force
-      then have "j' = count (transitions_of' (p, u, u_ss, p1)) t + count (transitions_of' (q', v, v_ss, q)) t"
+      then have "j' = count (transitions_of' (Ctr_Loc p, u, u_ss, Ctr_Loc p1)) t + count (transitions_of' (q', v, v_ss, q)) t"
         by auto
       then have "j' = 0 + count (transitions_of' (q', v, v_ss, q)) t"
         using avoid_count_zero
         by (metis p1_\<gamma>_p2_w2_q'_p(4) t_def u_v_u_ss_v_ss_p(2))
-      then have xx: "j' = count (transitions_of' (p2, op_labels w2, w2_ss, q')) t  + count (transitions_of' (q', v, v_ss, q)) t"
+      then have xx: "j' = count (transitions_of' (Ctr_Loc p2, op_labels w2, w2_ss, q')) t  + count (transitions_of' (q', v, v_ss, q)) t"
         using V avoid_count_zero p1_\<gamma>_p2_w2_q'_p(4) t_def by fastforce 
-      then show "j' = count (transitions_of' (p2, w2v, w2v_ss, q)) t"
+      then show "j' = count (transitions_of' (Ctr_Loc p2, w2v, w2v_ss, q)) t"
       proof -
         have l_w2_ss: "length w2_ss = Suc (length (op_labels w2))" 
           by (meson III_2 LTS.transition_star_states_length)
@@ -661,22 +662,22 @@ next
           using LTS.transition_star_states.cases V(2) by force
         have last_hd: "last w2_ss = hd v_ss"
           by (metis III_2 LTS.transition_star_states_last V(2) LTS.transition_star_states_hd)
-        have "count (transitions_of' ((p2, op_labels w2, w2_ss, q') @@\<acute> (q', v, v_ss, q))) (p1, \<gamma>, q')
-          = count (transitions_of' (p2, w2v, w2v_ss, q))  (p1, \<gamma>, q')"
+        have "count (transitions_of' ((Ctr_Loc p2, op_labels w2, w2_ss, q') @@\<acute> (q', v, v_ss, q))) (Ctr_Loc p1, \<gamma>, q')
+          = count (transitions_of' (Ctr_Loc p2, w2v, w2v_ss, q)) (Ctr_Loc p1, \<gamma>, q')"
           by (simp add: w2v_def w2v_ss_def)
-        then have "count (transitions_of' (p2, w2v, w2v_ss, q))  (p1, \<gamma>, q') = count (transitions_of' (p2, op_labels w2, w2_ss, q'))  (p1, \<gamma>, q') + count (transitions_of' (q', v, v_ss, q))  (p1, \<gamma>, q')"
-          using count_append_transition_star_states[of w2_ss "op_labels w2" v_ss p2 q' q' v q p1 \<gamma> q' ]
+        then have "count (transitions_of' (Ctr_Loc p2, w2v, w2v_ss, q))  (Ctr_Loc p1, \<gamma>, q') = count (transitions_of' (Ctr_Loc p2, op_labels w2, w2_ss, q')) (Ctr_Loc p1, \<gamma>, q') + count (transitions_of' (q', v, v_ss, q)) (Ctr_Loc p1, \<gamma>, q')"
+          using count_append_transition_star_states[of w2_ss "op_labels w2" v_ss "Ctr_Loc p2" q' q' v q "Ctr_Loc p1" \<gamma> q']
           by (simp add: l_w2_ss v_ss_non_empty last_hd) 
-        then have "count (transitions_of' (p2, w2v, w2v_ss, q)) t = count (transitions_of' (p2, op_labels w2, w2_ss, q')) t + count (transitions_of' (q', v, v_ss, q)) t"
+        then have "count (transitions_of' (Ctr_Loc p2, w2v, w2v_ss, q)) t = count (transitions_of' (Ctr_Loc p2, op_labels w2, w2_ss, q')) t + count (transitions_of' (q', v, v_ss, q)) t"
           using t_def by auto
         then show ?thesis
           using xx by auto
       qed
     qed
 
-    have "\<exists>p' w' ss'. (p', w', ss', q) \<in> LTS.transition_star_states A \<and> (p2, w2v) \<Rightarrow>\<^sup>* (p', w')"
+    have "\<exists>p' w' ss'. (Ctr_Loc p', w', ss', q) \<in> LTS.transition_star_states A \<and> (p2, w2v) \<Rightarrow>\<^sup>* (p', w')"
       using Suc(1) using j'_count V_merged by auto
-    then obtain p' w' ss' where p'_w'_ss'_p: "(p', w', ss', q) \<in> LTS.transition_star_states A" "(p2, w2v) \<Rightarrow>\<^sup>* (p', w')"
+    then obtain p' w' ss' where p'_w'_ss'_p: "(Ctr_Loc p', w', ss', q) \<in> LTS.transition_star_states A" "(p2, w2v) \<Rightarrow>\<^sup>* (p', w')"
       by blast
 
     note X = p'_w'_ss'_p(2)
@@ -703,7 +704,7 @@ next
     have "(p, w) \<Rightarrow>\<^sup>* (p', w')"
       using X \<open>(p, u @ [\<gamma>] @ v) \<Rightarrow>\<^sup>* (p1, \<gamma> # v)\<close> \<open>(p, w) = (p, u @ [\<gamma>] @ v)\<close> \<open>(p1, \<gamma> # v) \<Rightarrow> (p2, w2v)\<close> by auto
 
-    then have "(p', w', ss', q) \<in> LTS.transition_star_states A \<and> (p, w) \<Rightarrow>\<^sup>* (p', w')"
+    then have "(Ctr_Loc p', w', ss', q) \<in> LTS.transition_star_states A \<and> (p, w) \<Rightarrow>\<^sup>* (p', w')"
       using p'_w'_ss'_p(1) by auto
     then show ?case
       by metis
@@ -711,24 +712,24 @@ next
 qed 
 
 lemma lemma_3_2_a'':
-  assumes "\<nexists>q \<gamma> q'. (q, \<gamma>, q') \<in> A \<and> q' \<in> P_locs"
+  assumes "\<nexists>q \<gamma> q'. (q, \<gamma>, Ctr_Loc q') \<in> A"
   assumes "pre_star_rule\<^sup>*\<^sup>* A A'"
-  assumes "(p, w, q) \<in> LTS.transition_star A'"
-  shows "\<exists>p' w' ss'. (p', w', q) \<in> LTS.transition_star A \<and> (p, w) \<Rightarrow>\<^sup>* (p', w')"
+  assumes "(Ctr_Loc p, w, q) \<in> LTS.transition_star A'"
+  shows "\<exists>p' w' ss'. (Ctr_Loc p', w', q) \<in> LTS.transition_star A \<and> (p, w) \<Rightarrow>\<^sup>* (p', w')"
   using lemma_3_2_a' assms
   by (meson LTS.transition_star_states_transition_star LTS.transition_star_transition_star_states)
 
 lemma lemma_3_2_a:
-  assumes "\<nexists>q \<gamma> q'. (q, \<gamma>, q') \<in> A \<and> q' \<in> P_locs"
+  assumes "\<nexists>q \<gamma> q'. (q, \<gamma>, Ctr_Loc q') \<in> A"
   assumes "saturation pre_star_rule A A'"
-  assumes "(p, w, q) \<in> LTS.transition_star A'"
-  shows "\<exists>p' w'. (p', w', q) \<in> LTS.transition_star A \<and> (p, w) \<Rightarrow>\<^sup>* (p', w')"
+  assumes "(Ctr_Loc p, w, q) \<in> LTS.transition_star A'"
+  shows "\<exists>p' w'. (Ctr_Loc p', w', q) \<in> LTS.transition_star A \<and> (p, w) \<Rightarrow>\<^sup>* (p', w')"
   using assms lemma_3_2_a'' saturation_def by metis 
 
 lemmas lemma_3_2 = lemma_3_2_a lemma_3_2_b
 
 theorem theorem_3_2:
-  assumes "\<nexists>q \<gamma> q'. (q, \<gamma>, q') \<in> A \<and> q' \<in> P_locs"
+  assumes "\<nexists>q \<gamma> q'. (q, \<gamma>, Ctr_Loc q') \<in> A"
   assumes "saturation pre_star_rule A A'"
   shows "{c. accepts A' c} = pre_star (language A)"
 proof (rule; rule)
@@ -742,7 +743,7 @@ proof (rule; rule)
     unfolding pre_star_def by force
   then obtain p' w' where "(p',w') \<in> language A \<and> (p,w) \<Rightarrow>\<^sup>* (p',w')"
     by auto
-  then have "\<exists>q \<in> F_locs. (p, w, q) \<in> LTS.transition_star A'"
+  then have "\<exists>q \<in> F_locs. (Ctr_Loc p, w, q) \<in> LTS.transition_star A'"
     using lemma_3_1 assms(2) unfolding accepts_def by force
   then have "accepts A' (p,w)"
     unfolding accepts_def by auto
@@ -755,13 +756,13 @@ next
   define w where "w = snd c"
   from p_def w_def c_a have "accepts A' (p,w)"
     by auto
-  then have "\<exists>q \<in> F_locs. (p, w, q) \<in> LTS.transition_star A'"
+  then have "\<exists>q \<in> F_locs. (Ctr_Loc p, w, q) \<in> LTS.transition_star A'"
     unfolding accepts_def by auto
-  then obtain q where q_p: "q \<in> F_locs" "(p, w, q) \<in> LTS.transition_star A'"
+  then obtain q where q_p: "q \<in> F_locs" "(Ctr_Loc p, w, q) \<in> LTS.transition_star A'"
     by auto
-  then have "\<exists>p' w'. (p,w) \<Rightarrow>\<^sup>* (p',w') \<and> (p', w', q) \<in> LTS.transition_star A"
+  then have "\<exists>p' w'. (p,w) \<Rightarrow>\<^sup>* (p',w') \<and> (Ctr_Loc p', w', q) \<in> LTS.transition_star A"
     using lemma_3_2_a assms(1) assms(2) by metis
-  then obtain p' w' where p'_w'_p: "(p,w) \<Rightarrow>\<^sup>* (p',w')" "(p', w', q) \<in> LTS.transition_star A"
+  then obtain p' w' where p'_w'_p: "(p,w) \<Rightarrow>\<^sup>* (p',w')" "(Ctr_Loc p', w', q) \<in> LTS.transition_star A"
     by auto
   then have "(p', w') \<in> language A"
     unfolding language_def unfolding accepts_def using q_p(1) by auto
@@ -774,12 +775,11 @@ qed
 
 subsection \<open>Post* lemmas\<close>
 
-
-lemma lemma_3_3:
+lemma lemma_3_3':
   assumes "pv \<Rightarrow>\<^sup>* p'w"
-    and "(Ctr_Loc (fst pv), snd pv) \<in> language_\<epsilon> A"
+    and "(fst pv, snd pv) \<in> language_\<epsilon> A"
     and "saturation post_star_rules A A'"
-  shows "accepts_\<epsilon> A' (Ctr_Loc (fst p'w), snd p'w)"
+  shows "accepts_\<epsilon> A' (fst p'w, snd p'w)"
   using assms
 proof (induct arbitrary: pv rule: rtranclp_induct)
   case base
@@ -797,41 +797,41 @@ next
   have p''u_def: "p''u = (p'', u)"
     using p''_def u_def by auto
 
-  then have "accepts_\<epsilon> A' (Ctr_Loc p'', u)"
+  then have "accepts_\<epsilon> A' (p'', u)"
     using assms(2) p''_def step.hyps(3) step.prems(2) u_def by metis
-  then obtain q where q_p: "q \<in> F_locs \<and> (Ctr_Loc p'', u, Ctr_Loc q) \<in> LTS_\<epsilon>.transition_star_\<epsilon> A'"
+  then obtain q where q_p: "q \<in> F_locs \<and> (Ctr_Loc p'', u, q) \<in> LTS_\<epsilon>.transition_star_\<epsilon> A'"
     by (smt (verit, ccfv_threshold) accepts_\<epsilon>_def case_prod_conv)
-  then obtain u_\<epsilon> where II: "q \<in> F_locs" "LTS_\<epsilon>.\<epsilon>_exp u_\<epsilon> u" "(Ctr_Loc p'', u_\<epsilon>, Ctr_Loc q) \<in> LTS.transition_star A'"
-    using LTS_\<epsilon>.epsilon_lemma3[of "Ctr_Loc p''" u "Ctr_Loc q" A'] by auto
+  then obtain u_\<epsilon> where II: "q \<in> F_locs" "LTS_\<epsilon>.\<epsilon>_exp u_\<epsilon> u" "(Ctr_Loc p'', u_\<epsilon>, q) \<in> LTS.transition_star A'"
+    using LTS_\<epsilon>.epsilon_lemma3[of "Ctr_Loc p''" u q A'] by auto
   have "\<exists>\<gamma> u1 w1. u=\<gamma>#u1 \<and> w=op_labels w1@u1 \<and> (p'', \<gamma>) \<hookrightarrow> (p', w1)"
     using p''u_def p'w_def step.hyps(2) step_relp_def2 by auto
   then obtain \<gamma> u1 w1 where III: "u=\<gamma>#u1" " w=op_labels w1@u1" "(p'', \<gamma>) \<hookrightarrow> (p', w1)"
     by blast
 
-  have p'_P_locs: "p' \<in> P_locs"
-    using p''u_def p'w_def step.hyps(2) step_relp'_P_locs2 by blast
-  have p''_P_locs: "p'' \<in> P_locs"
-    using p''u_def p'w_def step.hyps(2) step_relp'_P_locs1 by blast
+  have p'_P_locs: "Ctr_Loc p' \<in> P_locs"
+    unfolding P_locs_def by auto
+  have p''_P_locs: "Ctr_Loc p'' \<in> P_locs"
+    unfolding P_locs_def by auto
 
-  have "\<exists>\<gamma>_\<epsilon> u1_\<epsilon>. LTS_\<epsilon>.\<epsilon>_exp \<gamma>_\<epsilon> [\<gamma>] \<and> LTS_\<epsilon>.\<epsilon>_exp u1_\<epsilon> u1 \<and> (Ctr_Loc p'', \<gamma>_\<epsilon>@u1_\<epsilon>, Ctr_Loc q) \<in> LTS.transition_star A'"
+  have "\<exists>\<gamma>_\<epsilon> u1_\<epsilon>. LTS_\<epsilon>.\<epsilon>_exp \<gamma>_\<epsilon> [\<gamma>] \<and> LTS_\<epsilon>.\<epsilon>_exp u1_\<epsilon> u1 \<and> (Ctr_Loc p'', \<gamma>_\<epsilon>@u1_\<epsilon>, q) \<in> LTS.transition_star A'"
   proof -
     have "\<exists>\<gamma>_\<epsilon> u1_\<epsilon>. LTS_\<epsilon>.\<epsilon>_exp \<gamma>_\<epsilon> [\<gamma>] \<and> LTS_\<epsilon>.\<epsilon>_exp u1_\<epsilon> u1 \<and> u_\<epsilon> = \<gamma>_\<epsilon> @ u1_\<epsilon>" 
       using LTS_\<epsilon>.\<epsilon>_exp_split'[of u_\<epsilon> \<gamma> u1] II(2) III(1) by auto
     then obtain \<gamma>_\<epsilon> u1_\<epsilon> where "LTS_\<epsilon>.\<epsilon>_exp \<gamma>_\<epsilon> [\<gamma>] \<and> LTS_\<epsilon>.\<epsilon>_exp u1_\<epsilon> u1 \<and> u_\<epsilon> = \<gamma>_\<epsilon> @ u1_\<epsilon>" 
       by auto
-    then have "(Ctr_Loc p'', \<gamma>_\<epsilon>@u1_\<epsilon> , Ctr_Loc q) \<in> LTS.transition_star A'"
+    then have "(Ctr_Loc p'', \<gamma>_\<epsilon>@u1_\<epsilon> , q) \<in> LTS.transition_star A'"
       using II(3) by auto
     then show ?thesis
       using \<open>LTS_\<epsilon>.\<epsilon>_exp \<gamma>_\<epsilon> [\<gamma>] \<and> LTS_\<epsilon>.\<epsilon>_exp u1_\<epsilon> u1 \<and> u_\<epsilon> = \<gamma>_\<epsilon> @ u1_\<epsilon>\<close> by blast
   qed
-  then obtain \<gamma>_\<epsilon> u1_\<epsilon> where iii: "LTS_\<epsilon>.\<epsilon>_exp \<gamma>_\<epsilon> [\<gamma>]" and iv: "LTS_\<epsilon>.\<epsilon>_exp u1_\<epsilon> u1" "(Ctr_Loc p'', \<gamma>_\<epsilon>@u1_\<epsilon>, Ctr_Loc q) \<in> LTS.transition_star A'"
+  then obtain \<gamma>_\<epsilon> u1_\<epsilon> where iii: "LTS_\<epsilon>.\<epsilon>_exp \<gamma>_\<epsilon> [\<gamma>]" and iv: "LTS_\<epsilon>.\<epsilon>_exp u1_\<epsilon> u1" "(Ctr_Loc p'', \<gamma>_\<epsilon>@u1_\<epsilon>, q) \<in> LTS.transition_star A'"
     by blast
-  then have VI: "\<exists>q1. (Ctr_Loc p'', \<gamma>_\<epsilon>, q1) \<in> LTS.transition_star A' \<and> (q1, u1_\<epsilon>, Ctr_Loc q) \<in> LTS.transition_star A'"
+  then have VI: "\<exists>q1. (Ctr_Loc p'', \<gamma>_\<epsilon>, q1) \<in> LTS.transition_star A' \<and> (q1, u1_\<epsilon>, q) \<in> LTS.transition_star A'"
     by (simp add: LTS.transition_star_split)
-  then obtain q1 where VI: "(Ctr_Loc p'', \<gamma>_\<epsilon>, q1) \<in> LTS.transition_star A'" "(q1, u1_\<epsilon>, Ctr_Loc q) \<in> LTS.transition_star A'"
+  then obtain q1 where VI: "(Ctr_Loc p'', \<gamma>_\<epsilon>, q1) \<in> LTS.transition_star A'" "(q1, u1_\<epsilon>, q) \<in> LTS.transition_star A'"
     by blast
 
-  then have VI_2: "(Ctr_Loc p'', [\<gamma>], q1) \<in> LTS_\<epsilon>.transition_star_\<epsilon> A'" "(q1, u1, Ctr_Loc q) \<in> LTS_\<epsilon>.transition_star_\<epsilon> A'"
+  then have VI_2: "(Ctr_Loc p'', [\<gamma>], q1) \<in> LTS_\<epsilon>.transition_star_\<epsilon> A'" "(q1, u1, q) \<in> LTS_\<epsilon>.transition_star_\<epsilon> A'"
      apply (meson LTS_\<epsilon>.epsilon_lemma3 iii)
     apply (meson LTS_\<epsilon>.epsilon_lemma3 VI(2) iv(1))
     done
@@ -843,9 +843,9 @@ next
       using III(3) by blast
     then have "(Ctr_Loc p', \<epsilon>, q1) \<in> A'"
       using VI_2(1) add_trans_pop assms saturated_def saturation_def p'_P_locs by metis
-    then have "(Ctr_Loc p', w, Ctr_Loc q) \<in> LTS_\<epsilon>.transition_star_\<epsilon> A'"
+    then have "(Ctr_Loc p', w, q) \<in> LTS_\<epsilon>.transition_star_\<epsilon> A'"
       using III(2)  VI_2(2) pop LTS_\<epsilon>.transition_star_\<epsilon>.transition_star_\<epsilon>_step_\<epsilon> by fastforce
-    then have "accepts_\<epsilon> A' (Ctr_Loc p', w)"
+    then have "accepts_\<epsilon> A' (p', w)"
       unfolding accepts_\<epsilon>_def
       using II(1) by blast
     then show ?thesis
@@ -856,10 +856,10 @@ next
       using III(3) by blast
     then have "(Ctr_Loc p', Some \<gamma>', q1) \<in> A'"
       by (metis VI_2(1) add_trans_swap assms(3) saturated_def saturation_def)
-    have "(Ctr_Loc p', w, Ctr_Loc q) \<in> LTS_\<epsilon>.transition_star_\<epsilon> A'"
+    have "(Ctr_Loc p', w, q) \<in> LTS_\<epsilon>.transition_star_\<epsilon> A'"
       using III(2) LTS_\<epsilon>.transition_star_\<epsilon>.transition_star_\<epsilon>_step_\<gamma> VI_2(2) append_Cons append_self_conv2 op_labels.simps(3) swap
       using \<open>(Ctr_Loc p', Some \<gamma>', q1) \<in> A'\<close> by fastforce
-    then have "accepts_\<epsilon> A' (Ctr_Loc p', w)"
+    then have "accepts_\<epsilon> A' (p', w)"
       unfolding accepts_\<epsilon>_def
       using II(1) by blast
     then show ?thesis
@@ -873,11 +873,11 @@ next
     from this r VI_2 iii post_star_rules.intros(4)[OF r, of q1 A', OF VI_2(1)] have "(Ctr_Loc_Ext p' \<gamma>', Some \<gamma>'', q1) \<in> A'"
       using assms(3) using saturated_def saturation_def
       by metis
-    have "(Ctr_Loc p', [\<gamma>'], Ctr_Loc_Ext p' \<gamma>') \<in> LTS_\<epsilon>.transition_star_\<epsilon> A' \<and> (Ctr_Loc_Ext p' \<gamma>', [\<gamma>''], q1) \<in> LTS_\<epsilon>.transition_star_\<epsilon> A' \<and> (q1, u1, Ctr_Loc q) \<in> LTS_\<epsilon>.transition_star_\<epsilon> A'"
+    have "(Ctr_Loc p', [\<gamma>'], Ctr_Loc_Ext p' \<gamma>') \<in> LTS_\<epsilon>.transition_star_\<epsilon> A' \<and> (Ctr_Loc_Ext p' \<gamma>', [\<gamma>''], q1) \<in> LTS_\<epsilon>.transition_star_\<epsilon> A' \<and> (q1, u1, q) \<in> LTS_\<epsilon>.transition_star_\<epsilon> A'"
       by (metis LTS_\<epsilon>.transition_star_\<epsilon>.simps VI_2(2) \<open>(Ctr_Loc p', Some \<gamma>', Ctr_Loc_Ext p' \<gamma>') \<in> A'\<close> \<open>(Ctr_Loc_Ext p' \<gamma>', Some \<gamma>'', q1) \<in> A'\<close>)
-    have "(Ctr_Loc p', w, Ctr_Loc q) \<in> LTS_\<epsilon>.transition_star_\<epsilon> A'"
+    have "(Ctr_Loc p', w, q) \<in> LTS_\<epsilon>.transition_star_\<epsilon> A'"
       by (smt (z3) III(2) LTS_\<epsilon>.transition_star_\<epsilon>.transition_star_\<epsilon>_step_\<gamma> VI_2(2) \<open>(Ctr_Loc p', Some \<gamma>', Ctr_Loc_Ext p' \<gamma>') \<in> A'\<close> \<open>(Ctr_Loc_Ext p' \<gamma>', Some \<gamma>'', q1) \<in> A'\<close> append_Cons append_self_conv2 op_labels.simps(3) push)
-    then have "accepts_\<epsilon> A' (Ctr_Loc p', w)"
+    then have "accepts_\<epsilon> A' (p', w)"
       unfolding accepts_\<epsilon>_def
       using II(1) by blast
     then show ?thesis
@@ -885,6 +885,13 @@ next
 
   qed
 qed
+
+lemma lemma_3_3:
+  assumes "(p,v) \<Rightarrow>\<^sup>* (p',w)"
+    and "(p, v) \<in> language_\<epsilon> A"
+    and "saturation post_star_rules A A'"
+  shows "accepts_\<epsilon> A' (p', w)"
+  using assms lemma_3_3' by force
 
 thm lemma_3_2_a'
 term LTS_\<epsilon>.remove_\<epsilon>
@@ -947,11 +954,10 @@ lemma transition_list_Cons:
 
 lemma xxxxxxxxxx:
   assumes "(ss, w) \<in> LTS.path_with_word A"
-  assumes "\<nexists>q \<gamma> q'. (q, \<gamma>, Ctr_Loc q') \<in> A \<and> q' \<in> P_locs"
+  assumes "\<nexists>q \<gamma> q'. (q, \<gamma>, Ctr_Loc q') \<in> A"
   assumes "t = (Ctr_Loc p1, \<gamma>, q1)"
-  assumes "p1 \<in> P_locs"
   shows "count (transitions_of (ss, w)) t = 0 \<or> ((hd (transition_list (ss, w)) = t \<and> count (transitions_of (ss, w)) t = 1))"
-  using assms 
+  using assms
 proof (induction rule: LTS.path_with_word.induct[OF assms(1)])
   case (1 s)
   then show ?case
@@ -990,18 +996,17 @@ qed
 
 lemma xxxxxxxxxxxxxxx:
   assumes "(ss, w) \<in> LTS.path_with_word A"
-  assumes "\<nexists>q \<gamma> q'. (q, \<gamma>, Ctr_Loc q') \<in> A \<and> q' \<in> P_locs"
+  assumes "\<nexists>q \<gamma> q'. (q, \<gamma>, Ctr_Loc q') \<in> A"
   assumes "count (transitions_of (ss, w)) t > 0"
   assumes "t = (Ctr_Loc p1, \<gamma>, q1)"
-  assumes "p1 \<in> P_locs"
   shows "hd (transition_list (ss, w)) = t \<and> count (transitions_of (ss, w)) t = 1"
   using xxxxxxxxxx assms by (metis not_gr_zero)
 
 lemma help''''':
   assumes "hd (transition_list (ss, w)) = t"
   assumes "transition_list (ss, w) \<noteq> []"
-  assumes "t = (Ctr_Loc p1, \<gamma>, q1)"
-  shows  "([Ctr_Loc p1, q1], [\<gamma>]) @\<acute> (tl ss, tl w) = (ss, w)"
+  assumes "t = (p1, \<gamma>, q1)"
+  shows  "([p1, q1], [\<gamma>]) @\<acute> (tl ss, tl w) = (ss, w)"
   using assms apply simp
   apply (cases ss; cases w)
      apply auto
@@ -1022,9 +1027,9 @@ lemma help''''':
 find_theorems pre_star_rule P_locs
 
 lemma agagagagagaga:
-  assumes "(p, w, Ctr_Loc qq) \<in> LTS.transition_star Aiminus1"
+  assumes "(p, w, qq) \<in> LTS.transition_star Aiminus1"
   assumes "w \<noteq> []"
-  assumes "\<nexists>q \<gamma> q'. (q, \<gamma>, Ctr_Loc q') \<in> Aiminus1 \<and> q' \<in> P_locs"
+  assumes "\<nexists>q \<gamma> q'. (q, \<gamma>, Ctr_Loc q') \<in> Aiminus1"
   shows "qq \<notin> P_locs"
   using assms
 proof (induction rule: LTS.transition_star.induct[OF assms(1)])
@@ -1034,19 +1039,19 @@ proof (induction rule: LTS.transition_star.induct[OF assms(1)])
 next
   case (2 p \<gamma> q' w q)
   then show ?case
-    by (metis LTS.transition_star.cases LTS.transition_star_transition_star_states LTS.xxxxxxx assms(1) assms(2))
+    by (metis LTS.transition_star_empty P_locs_def is_Ctr_Loc_def mem_Collect_eq)
 qed
 
 
 lemma agagagagagaga'''':
-  assumes "(p, [\<gamma>], Ctr_Loc qq) \<in> LTS_\<epsilon>.transition_star_\<epsilon> Aiminus1"
-  assumes "(p', \<epsilon>, Ctr_Loc qq) \<notin> Aiminus1"
-  assumes "\<nexists>q \<gamma> q'. (q, \<gamma>, Ctr_Loc q') \<in> Aiminus1 \<and> q' \<in> P_locs"
+  assumes "(p, [\<gamma>], qq) \<in> LTS_\<epsilon>.transition_star_\<epsilon> Aiminus1"
+  assumes "(p', \<epsilon>, qq) \<notin> Aiminus1"
+  assumes "\<nexists>q \<gamma> q'. (q, \<gamma>, Ctr_Loc q') \<in> Aiminus1"
   shows "qq \<notin> P_locs"
 proof -
-  have "\<exists>w. LTS_\<epsilon>.\<epsilon>_exp w [\<gamma>] \<and> (p, w, Ctr_Loc qq) \<in> LTS.transition_star Aiminus1 \<and> w \<noteq> []"
+  have "\<exists>w. LTS_\<epsilon>.\<epsilon>_exp w [\<gamma>] \<and> (p, w, qq) \<in> LTS.transition_star Aiminus1 \<and> w \<noteq> []"
     by (metis (no_types, hide_lams) LTS_\<epsilon>.\<epsilon>_exp_def LTS_\<epsilon>.\<epsilon>_exp_split' LTS_\<epsilon>.epsilon_lemma3 append_Cons append_Nil assms(1) list.distinct(1) list.exhaust)
-  then obtain w where "LTS_\<epsilon>.\<epsilon>_exp w [\<gamma>] \<and> (p, w, Ctr_Loc qq) \<in> LTS.transition_star Aiminus1 \<and> w \<noteq> []"
+  then obtain w where "LTS_\<epsilon>.\<epsilon>_exp w [\<gamma>] \<and> (p, w, qq) \<in> LTS.transition_star Aiminus1 \<and> w \<noteq> []"
     by blast
   then show ?thesis
     using agagagagagaga[of p w qq Aiminus1] assms(3) by auto
@@ -1054,73 +1059,49 @@ qed
 
 lemma agagagagagaga''''''''':
   assumes "post_star_rules\<^sup>*\<^sup>* A Ai"
-  assumes "\<nexists>q \<gamma> q'. (q, \<gamma>, Ctr_Loc q') \<in> A \<and> q' \<in> P_locs"
-  shows "\<nexists>q \<gamma> q'. (q, \<gamma>, Ctr_Loc q') \<in> Ai \<and> q' \<in> P_locs"
+  assumes "\<nexists>q \<gamma> q'. (q, \<gamma>, Ctr_Loc q') \<in> A"
+  shows "\<nexists>q \<gamma> q'. (q, \<gamma>, Ctr_Loc q') \<in> Ai"
 using assms 
 proof (induction rule: rtranclp_induct)
   case base
   then show ?case by auto
 next
   case (step Aiminus1 Ai)
-  then have ind: "\<nexists>q \<gamma> q'. (q, \<gamma>, Ctr_Loc q') \<in> Aiminus1 \<and> q' \<in> P_locs"
+  then have ind: "\<nexists>q \<gamma> q'. (q, \<gamma>, Ctr_Loc q') \<in> Aiminus1"
     by auto
   from step(2) show ?case
   proof (cases rule: post_star_rules.cases)
     case (add_trans_pop p \<gamma> p' q)
+    have "q \<notin> P_locs"
+      using add_trans_pop ind agagagagagaga'''' by blast 
+    then have "\<nexists>qq. q = Ctr_Loc qq"
+      by (simp add: P_locs_def is_Ctr_Loc_def)
     then show ?thesis
-    proof (cases q)
-      case (Ctr_Loc qq)
-      have "qq \<notin> P_locs"
-        using add_trans_pop ind agagagagagaga'''' Ctr_Loc by blast 
-      then show ?thesis
-        using Ctr_Loc ind add_trans_pop(1) by fastforce
-    next
-      case (Ctr_Loc_Ext qq ll)
-      then show ?thesis
-        using add_trans_pop step(3) ind by auto
-    qed
+      using ind local.add_trans_pop(1) by auto
   next
     case (add_trans_swap p \<gamma> p' \<gamma>' q)
+    have "q \<notin> P_locs"
+      using add_trans_swap ind agagagagagaga'''' by (metis P_locs_def is_Ctr_Loc_def mem_Collect_eq)
+    then have "\<nexists>qq. q = Ctr_Loc qq"
+      by (simp add: P_locs_def is_Ctr_Loc_def)
     then show ?thesis
-    proof (cases q)
-      case (Ctr_Loc qq)
-      have "qq \<notin> P_locs"
-        using add_trans_swap ind agagagagagaga'''' Ctr_Loc by blast 
-      then show ?thesis
-        using Ctr_Loc ind add_trans_swap(1) by fastforce
-    next
-      case (Ctr_Loc_Ext qq ll)
-      then show ?thesis
-        using add_trans_swap step(3) ind by auto
-    qed
+      using ind local.add_trans_swap(1) by auto
   next
     case (add_trans_push_1 p \<gamma> p' \<gamma>' \<gamma>'' q)
-    then show ?thesis 
-    proof (cases q)
-      case (Ctr_Loc qq)
-      have "qq \<notin> P_locs"
-        using add_trans_push_1 ind agagagagagaga'''' Ctr_Loc by blast 
-      then show ?thesis
-        using Ctr_Loc ind add_trans_push_1(1) by fastforce
-    next
-      case (Ctr_Loc_Ext qq ll)
-      then show ?thesis
-        using add_trans_push_1 step(3) ind by auto
-    qed
+    have "q \<notin> P_locs"
+      using add_trans_push_1 ind agagagagagaga''''  by (metis P_locs_def is_Ctr_Loc_def mem_Collect_eq)
+    then have "\<nexists>qq. q = Ctr_Loc qq"
+      by (simp add: P_locs_def is_Ctr_Loc_def)
+    then show ?thesis
+      using ind local.add_trans_push_1(1) by auto
   next
     case (add_trans_push_2 p \<gamma> p' \<gamma>' \<gamma>'' q)
-    then show ?thesis 
-    proof (cases q)
-      case (Ctr_Loc qq)
-      have "qq \<notin> P_locs"
-        using add_trans_push_2 ind agagagagagaga'''' Ctr_Loc by blast 
-      then show ?thesis
-        using Ctr_Loc ind add_trans_push_2(1) by fastforce
-    next
-      case (Ctr_Loc_Ext qq ll)
-      then show ?thesis
-        using add_trans_push_2 step(3) ind by auto
-    qed
+    have "q \<notin> P_locs"
+      using add_trans_push_2 ind agagagagagaga''''  by (metis P_locs_def is_Ctr_Loc_def mem_Collect_eq)
+    then have "\<nexists>qq. q = Ctr_Loc qq"
+      by (simp add: P_locs_def is_Ctr_Loc_def)
+    then show ?thesis
+      using ind local.add_trans_push_2(1) by auto
   qed
 qed
 
@@ -1147,14 +1128,14 @@ qed
 
 lemma lemma_3_4'_Aux:
   assumes "post_star_rules\<^sup>*\<^sup>* A A'"
-  assumes "\<forall>a b c. (a, b, c) \<in> A \<longrightarrow> is_Ctr_Loc a \<and> is_Ctr_Loc c"
+  assumes "\<forall>a b c. (a, b, c) \<in> A \<longrightarrow> a \<notin> New_Aut_states \<and> c \<notin> New_Aut_states"
   assumes "(Ctr_Loc p', Some \<gamma>', Ctr_Loc_Ext p' \<gamma>') \<notin> A'"
   shows "\<nexists>p \<gamma>. (p, \<gamma>, Ctr_Loc_Ext p' \<gamma>') \<in> A'"
   using assms 
 proof (induction rule: rtranclp_induct)
   case base
   then show ?case 
-    by force
+    unfolding New_Aut_states_def is_Ctr_Ext_def by blast
 next
   case (step Aiminus1 Ai)
   from step(2) show ?case
@@ -1166,7 +1147,7 @@ next
       using local.add_trans_pop(1) step.IH step.prems(1) by fastforce
     then have "Ctr_Loc_Ext p' \<gamma>' \<noteq> q"
       using add_trans_pop(4) lemma_3_4'_Aux_Aux
-      by (metis ctr_loc.distinct(1))
+      by (metis local.add_trans_pop(3) state.distinct(3))
     then have "\<nexists>p \<gamma>. (p, \<gamma>, Ctr_Loc_Ext p' \<gamma>') = (Ctr_Loc p'', \<epsilon>, q)"
       by auto
     then show ?thesis
@@ -1178,7 +1159,7 @@ next
     then have nin: "\<nexists>p \<gamma>. (p, \<gamma>, Ctr_Loc_Ext p' \<gamma>') \<in> Aiminus1"
       using local.add_trans_swap(1) step.IH step.prems(1) by fastforce
     then have "Ctr_Loc_Ext p' \<gamma>' \<noteq> q"
-      by (metis ctr_loc.distinct(1) lemma_3_4'_Aux_Aux local.add_trans_swap(3)) 
+      by (metis state.distinct(4) lemma_3_4'_Aux_Aux local.add_trans_swap(3)) 
     then have "\<nexists>p \<gamma>. (p, \<gamma>, Ctr_Loc_Ext p' \<gamma>') = (Ctr_Loc p'', Some \<gamma>''', q)"
       by auto
     then show ?thesis
@@ -1189,7 +1170,7 @@ next
       using step.prems(2) by blast
     then show ?thesis
       using add_trans_push_1(1)
-      using Un_iff ctr_loc.inject(2) prod.inject singleton_iff step.IH step.prems(1) by blast 
+      using Un_iff state.inject(2) prod.inject singleton_iff step.IH step.prems(1) by blast 
   next
     case (add_trans_push_2 p'''' \<gamma>'' p'' \<gamma>''' \<gamma>'''' q)
     then have "(Ctr_Loc p', Some \<gamma>', Ctr_Loc_Ext p' \<gamma>') \<notin> Ai"
@@ -1197,7 +1178,7 @@ next
     then have nin: "\<nexists>p \<gamma>. (p, \<gamma>, Ctr_Loc_Ext p' \<gamma>') \<in> Aiminus1"
       using local.add_trans_push_2(1) step.IH step.prems(1) by fastforce
     then have "Ctr_Loc_Ext p' \<gamma>' \<noteq> q"
-      by (metis ctr_loc.disc(3) ctr_loc.discI(2) lemma_3_4'_Aux_Aux local.add_trans_push_2(3))
+      by (metis state.disc(1,3) lemma_3_4'_Aux_Aux local.add_trans_push_2(3))
     then have "\<nexists>p \<gamma>. (p, \<gamma>, Ctr_Loc_Ext p' \<gamma>') = (Ctr_Loc p'', \<epsilon>, q)"
       by auto
     then show ?thesis
@@ -1208,14 +1189,14 @@ qed
 
 lemma lemma_3_4'_Aux_Aux2:
   assumes "post_star_rules\<^sup>*\<^sup>* A A'"
-  assumes "\<forall>a b c. (a, b, c) \<in> A \<longrightarrow> is_Ctr_Loc a \<and> is_Ctr_Loc c"
+  assumes "\<forall>a b c. (a, b, c) \<in> A \<longrightarrow> a \<notin> New_Aut_states \<and> c \<notin> New_Aut_states"
   assumes "(Ctr_Loc p', Some \<gamma>', Ctr_Loc_Ext p' \<gamma>') \<notin> A'"
   shows "\<nexists>p \<gamma>. (Ctr_Loc_Ext p' \<gamma>', \<gamma>, p) \<in> A'"
   using assms 
 proof (induction rule: rtranclp_induct) (* I copy-pasted this prove from above and blindly adjusted it. So it may be a mess. *)
   case base
   then show ?case 
-    by force
+    unfolding New_Aut_states_def is_Ctr_Ext_def by blast
 next
   case (step Aiminus1 Ai)
   from step(2) show ?case
@@ -1227,7 +1208,8 @@ next
       using local.add_trans_pop(1) step.IH step.prems(1) by fastforce
     then have "Ctr_Loc_Ext p' \<gamma>' \<noteq> q"
       using add_trans_pop(4) lemma_3_4'_Aux_Aux[of "Ctr_Loc p'''" "[\<gamma>'']" q Aiminus1 "Ctr_Loc_Ext p' \<gamma>'"]
-      using PDS_with_P_automaton.lemma_3_4'_Aux PDS_with_P_automaton_axioms local.add_trans_pop(1) step.hyps(1) step.prems(1) step.prems(2) by blast
+      using PDS_with_P_automaton.lemma_3_4'_Aux local.add_trans_pop(1) step.hyps(1) step.prems(1) step.prems(2)
+      using UnI1 local.add_trans_pop(3) by blast 
     then have "\<nexists>p \<gamma>. (p, \<gamma>, Ctr_Loc_Ext p' \<gamma>') = (Ctr_Loc p'', \<epsilon>, q)"
       by auto
     then show ?thesis
@@ -1239,8 +1221,9 @@ next
     then have nin: "\<nexists>p \<gamma>. (Ctr_Loc_Ext p' \<gamma>', \<gamma>, p) \<in> Aiminus1"
       using local.add_trans_swap(1) step.IH step.prems(1) by fastforce
     then have "Ctr_Loc_Ext p' \<gamma>' \<noteq> q"
-      using ctr_loc.distinct(1) lemma_3_4'_Aux_Aux local.add_trans_swap(3)
-      by (metis PDS_with_P_automaton.lemma_3_4'_Aux PDS_with_P_automaton_axioms UnCI local.add_trans_swap(1) step.hyps(1) step.prems(1) step.prems(2)) 
+      using lemma_3_4'_Aux_Aux local.add_trans_swap(3)
+      using PDS_with_P_automaton.lemma_3_4'_Aux  UnCI local.add_trans_swap(1) step.hyps(1) step.prems(1) step.prems(2)
+      by (metis state.simps(7))
     then have "\<nexists>p \<gamma>. (p, \<gamma>, Ctr_Loc_Ext p' \<gamma>') = (Ctr_Loc p'', Some \<gamma>''', q)"
       by auto
     then show ?thesis
@@ -1251,7 +1234,7 @@ next
       using step.prems(2) by blast
     then show ?thesis
       using add_trans_push_1(1)
-      using Un_iff ctr_loc.inject(2) prod.inject singleton_iff step.IH step.prems(1) by blast 
+      using Un_iff state.inject prod.inject singleton_iff step.IH step.prems(1) by blast 
   next
     case (add_trans_push_2 p'''' \<gamma>'' p'' \<gamma>''' \<gamma>'''' q)
     then have "(Ctr_Loc p', Some \<gamma>', Ctr_Loc_Ext p' \<gamma>') \<notin> Ai"
@@ -1259,8 +1242,8 @@ next
     then have nin: "\<nexists>p \<gamma>. (Ctr_Loc_Ext p' \<gamma>', \<gamma>, p) \<in> Aiminus1"
       using local.add_trans_push_2(1) step.IH step.prems(1) by fastforce
     then have "Ctr_Loc_Ext p' \<gamma>' \<noteq> q"
-      using ctr_loc.disc(3) ctr_loc.discI(2) lemma_3_4'_Aux_Aux local.add_trans_push_2(3)
-      by (metis PDS_with_P_automaton.lemma_3_4'_Aux PDS_with_P_automaton_axioms UnCI local.add_trans_push_2(1) step.hyps(1) step.prems(1) step.prems(2)) 
+      using state.disc(3) lemma_3_4'_Aux_Aux local.add_trans_push_2(3)
+      using PDS_with_P_automaton.lemma_3_4'_Aux UnCI local.add_trans_push_2(1) step.hyps(1) step.prems(1) step.prems(2) by (metis state.discI(1))
     then have "\<nexists>p \<gamma>. (Ctr_Loc_Ext p' \<gamma>', \<gamma>, p) = (Ctr_Loc p'', \<epsilon>, q)"
       by auto
     then show ?thesis
@@ -1288,35 +1271,34 @@ next
 qed
 
 lemma lemma_3_4':
-  (* assumes "\<nexists>q \<gamma> q'. (q, \<gamma>, q') \<in> A \<and> q' \<in> P_locs" *)
   assumes "post_star_rules\<^sup>*\<^sup>* A A'"
-  assumes "\<nexists>q \<gamma> q'. (q, \<gamma>, Ctr_Loc q') \<in> A \<and> q' \<in> P_locs"
-  assumes "\<forall>a b c. (a, b, c) \<in> A \<longrightarrow> is_Ctr_Loc a \<and> is_Ctr_Loc c"
+  assumes "\<nexists>q \<gamma> q'. (q, \<gamma>, Ctr_Loc q') \<in> A"
+  assumes "\<forall>a b c. (a, b, c) \<in> A \<longrightarrow> a \<notin> New_Aut_states \<and> c \<notin> New_Aut_states"
   assumes "(Ctr_Loc p, w, ss, q) \<in> LTS.transition_star_states A'"
-  shows "(is_Ctr_Loc q \<longrightarrow> (\<exists>p' w'. (Ctr_Loc p', w', q) \<in> LTS_\<epsilon>.transition_star_\<epsilon> A \<and> (p',w') \<Rightarrow>\<^sup>* (p, LTS_\<epsilon>.remove_\<epsilon> w))) \<and>
+  shows "(\<not>is_Ctr_Ext q \<longrightarrow> (\<exists>p' w'. (Ctr_Loc p', w', q) \<in> LTS_\<epsilon>.transition_star_\<epsilon> A \<and> (p',w') \<Rightarrow>\<^sup>* (p, LTS_\<epsilon>.remove_\<epsilon> w))) \<and>
          (is_Ctr_Ext q \<longrightarrow> (the_Ext_Ctr_Loc q, [the_Ext_Label q]) \<Rightarrow>\<^sup>* (p, LTS_\<epsilon>.remove_\<epsilon> w))"
   using assms
 proof (induction arbitrary: p q w ss rule: rtranclp_induct)
   case base
-  have "is_Ctr_Loc q \<or> is_Ctr_Ext q"
-    by (meson ctr_loc.exhaust_disc)
-  then show ?case
-  proof
-    assume ctr_loc: "is_Ctr_Loc q"
+  {
+    assume ctr_loc: "is_Ctr_Loc q \<or> is_State q"
     then have "(Ctr_Loc p, LTS_\<epsilon>.remove_\<epsilon> w, q) \<in> LTS_\<epsilon>.transition_star_\<epsilon> A"
       using base using LTS_\<epsilon>.transition_star_states_transition_star_\<epsilon> by metis
     then have "\<exists>p' w'. (p', w', q) \<in> LTS_\<epsilon>.transition_star_\<epsilon> A"
       by auto
-    then show ?case
+    then have ?case
       using ctr_loc
       using \<open>(Ctr_Loc p, LTS_\<epsilon>.remove_\<epsilon> w, q) \<in> LTS_\<epsilon>.transition_star_\<epsilon> A\<close> by blast
-  next
+  }
+  moreover
+  {
     assume "is_Ctr_Ext q"
-    then show ?case
+    then have ?case
     proof (cases w)
       case Nil
       then have False using base
-        by (metis LTS.transition_star_empty LTS.transition_star_states_transition_star \<open>is_Ctr_Ext q\<close> ctr_loc.disc(3))
+        using LTS.transition_star_empty LTS.transition_star_states_transition_star \<open>is_Ctr_Ext q\<close>
+        by (metis state.disc(7))
       then show ?thesis
         by metis
     next
@@ -1326,11 +1308,14 @@ proof (induction arbitrary: p q w ss rule: rtranclp_induct)
       then have "\<exists>s \<gamma>'. (s, \<gamma>', q) \<in> A"
         using LTS.xxxxxxx by metis
       then have False
-        using \<open>is_Ctr_Ext q\<close> base.prems(2) by blast
+        using \<open>is_Ctr_Ext q\<close> base.prems(2) New_Aut_states_def by blast
       then show ?thesis
         by auto
     qed
-  qed
+  }
+  ultimately
+  show ?case
+   by (meson state.exhaust_disc)
 next
   case (step Aiminus1 Ai)
   from step(2) have "\<exists>p1 \<gamma> p2 w2 q1. Ai = Aiminus1 \<union> {(p1, \<gamma>, q1)} \<and> (p1, \<gamma>, q1) \<notin> Aiminus1"
@@ -1362,7 +1347,7 @@ next
       note VI = add_trans_pop(2)
       have t_def: "t = (Ctr_Loc p1, \<epsilon>, q1)"
         using local.add_trans_pop(1) local.add_trans_pop p1_\<gamma>_p2_w2_q'_p(1) t_def by blast
-      have init_Ai: "\<nexists>q \<gamma> q'. (q, \<gamma>, Ctr_Loc q') \<in> Ai \<and> q' \<in> P_locs"
+      have init_Ai: "\<nexists>q \<gamma> q'. (q, \<gamma>, Ctr_Loc q') \<in> Ai"
         using step(1,2) step(4)
         using agagagagagaga'''''''''
         by (meson r_into_rtranclp)
@@ -1371,7 +1356,7 @@ next
         have "(ss, w) \<in> LTS.path_with_word Ai"
           using Suc(3) LTS.askdjfklasjflksa by metis
         moreover 
-        have "\<nexists>q \<gamma> q'. (q, \<gamma>, Ctr_Loc q') \<in> Ai \<and> q' \<in> P_locs"
+        have "\<nexists>q \<gamma> q'. (q, \<gamma>, Ctr_Loc q') \<in> Ai"
           using init_Ai by auto
         moreover 
         have "0 < count (transitions_of (ss, w)) t"
@@ -1380,8 +1365,8 @@ next
         have "t = (Ctr_Loc p1, \<epsilon>, q1)"
           using t_def by auto
         moreover 
-        have "p1 \<in> P_locs"
-          by (simp add: III)
+        have "Ctr_Loc p1 \<in> P_locs"
+          by (simp add: P_locs_def)
         ultimately
         show "hd (transition_list (ss, w)) = t \<and> count (transitions_of (ss, w)) t = 1"
           using xxxxxxxxxxxxxxx[of ss w Ai t p1 \<epsilon> q1] by auto
@@ -1419,7 +1404,7 @@ next
           using local.add_trans_pop(1) by auto
         moreover
         have "(Ctr_Loc p1, \<epsilon>, q1) \<notin> Aiminus1"
-          by (simp add: local.add_trans_pop(5))
+          by (simp add: local.add_trans_pop)
         ultimately
         show "(Ctr_Loc p1, [\<epsilon>], [Ctr_Loc p1, q1], q1) \<in> LTS.transition_star_states Ai"
           by (meson LTS.transition_star_states.transition_star_states_refl LTS.transition_star_states.transition_star_states_step)
@@ -1471,17 +1456,17 @@ next
         using IIII_1 IIII_2 by (meson LTS.transition_star_states_append)
 
       from Suc(1)[of p2 "\<gamma>2' @ tl w" "ss2 @ (tl (tl ss))" q]
-      have V: "(is_Ctr_Loc q \<longrightarrow>
+      have V: "(\<not>is_Ctr_Ext q \<longrightarrow>
      (\<exists>p' w'. (Ctr_Loc p', w', q) \<in> LTS_\<epsilon>.transition_star_\<epsilon> A \<and> (p', w') \<Rightarrow>\<^sup>* (p2, LTS_\<epsilon>.remove_\<epsilon> (\<gamma>2' @ tl w)))) \<and>
     (is_Ctr_Ext q \<longrightarrow> (the_Ext_Ctr_Loc q, [the_Ext_Label q]) \<Rightarrow>\<^sup>* (p2, LTS_\<epsilon>.remove_\<epsilon> (\<gamma>2' @ tl w)))"
         using IIII
         using step.IH step.prems(1) step.prems(2) by blast
 
-      have "is_Ctr_Loc q \<or> is_Ctr_Ext q"
-        using ctr_loc.exhaust_disc by blast
+      have "\<not>is_Ctr_Ext q \<or> is_Ctr_Ext q"
+        using state.exhaust_disc by blast
       then show ?thesis
       proof
-        assume ctr_q: "is_Ctr_Loc q"
+        assume ctr_q: "\<not>is_Ctr_Ext q"
         then have "\<exists>p' w'. (Ctr_Loc p', w', q) \<in> LTS_\<epsilon>.transition_star_\<epsilon> A \<and> (p', w') \<Rightarrow>\<^sup>* (p2, LTS_\<epsilon>.remove_\<epsilon> (\<gamma>2' @ tl w))"
           using V by auto
         then obtain p' w' where
@@ -1502,7 +1487,7 @@ next
             by (metis Cons_eq_appendI LTS_\<epsilon>.remove_\<epsilon>_append_dist self_append_conv2) 
           from one two have "(p2,  \<gamma>2 # (LTS_\<epsilon>.remove_\<epsilon> (tl w))) \<Rightarrow>\<^sup>* (p, LTS_\<epsilon>.remove_\<epsilon> (tl w))"
             using  VIII
-            by (metis PDS.transition_rel.intros PDS_axioms append_self_conv2 op_labels.simps(1) r_into_rtranclp step_relp_def) (* VII *) 
+            by (metis PDS.transition_rel.intros append_self_conv2 op_labels.simps(1) r_into_rtranclp step_relp_def) (* VII *) 
           then have "(p2, LTS_\<epsilon>.remove_\<epsilon> (\<gamma>2' @ tl w)) \<Rightarrow>\<^sup>* (p, LTS_\<epsilon>.remove_\<epsilon> (tl w))"
             by (simp add: LTS_\<epsilon>.remove_\<epsilon>_append_dist \<gamma>2'_\<gamma>2)
           ultimately
@@ -1534,7 +1519,7 @@ next
       note VI = add_trans_swap(2)
       have t_def: "t = (Ctr_Loc p1, Some \<gamma>', q1)"
         using local.add_trans_swap(1) local.add_trans_swap p1_\<gamma>_p2_w2_q'_p(1) t_def by blast
-      have init_Ai: "\<nexists>q \<gamma> q'. (q, \<gamma>, Ctr_Loc q') \<in> Ai \<and> q' \<in> P_locs"
+      have init_Ai: "\<nexists>q \<gamma> q'. (q, \<gamma>, Ctr_Loc q') \<in> Ai"
         using step(1,2) step(4)
         using agagagagagaga'''''''''
         by (meson r_into_rtranclp)
@@ -1543,7 +1528,7 @@ next
         have "(ss, w) \<in> LTS.path_with_word Ai"
           using Suc(3) LTS.askdjfklasjflksa by metis
         moreover 
-        have "\<nexists>q \<gamma> q'. (q, \<gamma>, Ctr_Loc q') \<in> Ai \<and> q' \<in> P_locs"
+        have "\<nexists>q \<gamma> q'. (q, \<gamma>, Ctr_Loc q') \<in> Ai"
           using init_Ai by auto
         moreover 
         have "0 < count (transitions_of (ss, w)) t"
@@ -1553,8 +1538,8 @@ next
           using t_def
           by auto
         moreover 
-        have "p1 \<in> P_locs"
-          using III VI step_relp'_P_locs2 step_relp_def2 by blast
+        have "Ctr_Loc p1 \<in> P_locs"
+          using P_locs_def by force
         ultimately
         show "hd (transition_list (ss, w)) = t \<and> count (transitions_of (ss, w)) t = 1"
           using xxxxxxxxxxxxxxx[of ss w Ai t p1 _ q1] by auto
@@ -1643,17 +1628,17 @@ next
         using IIII_1 IIII_2 by (meson LTS.transition_star_states_append)
 
       from Suc(1)[of p2 "\<gamma>2' @ tl w" "ss2 @ (tl (tl ss))" q]
-      have V: "(is_Ctr_Loc q \<longrightarrow>
+      have V: "(\<not>is_Ctr_Ext q \<longrightarrow>
      (\<exists>p' w'. (Ctr_Loc p', w', q) \<in> LTS_\<epsilon>.transition_star_\<epsilon> A \<and> (p', w') \<Rightarrow>\<^sup>* (p2, LTS_\<epsilon>.remove_\<epsilon> (\<gamma>2' @ tl w)))) \<and>
     (is_Ctr_Ext q \<longrightarrow> (the_Ext_Ctr_Loc q, [the_Ext_Label q]) \<Rightarrow>\<^sup>* (p2, LTS_\<epsilon>.remove_\<epsilon> (\<gamma>2' @ tl w)))"
         using IIII
         using step.IH step.prems(1) step.prems(2) by blast
 
-      have "is_Ctr_Loc q \<or> is_Ctr_Ext q"
-        using ctr_loc.exhaust_disc by blast
+      have "\<not>is_Ctr_Ext q \<or> is_Ctr_Ext q"
+        using state.exhaust_disc by blast
       then show ?thesis
       proof
-        assume ctr_q: "is_Ctr_Loc q"
+        assume ctr_q: "\<not>is_Ctr_Ext q"
         then have "\<exists>p' w'. (Ctr_Loc p', w', q) \<in> LTS_\<epsilon>.transition_star_\<epsilon> A \<and> (p', w') \<Rightarrow>\<^sup>* (p2, LTS_\<epsilon>.remove_\<epsilon> (\<gamma>2' @ tl w))"
           using V by auto
         then obtain p' w' where
@@ -1674,7 +1659,7 @@ next
             by (metis Cons_eq_appendI LTS_\<epsilon>.remove_\<epsilon>_append_dist self_append_conv2) 
           from one two have "(p2,  \<gamma>2 # (LTS_\<epsilon>.remove_\<epsilon> (tl w))) \<Rightarrow>\<^sup>* (p, \<gamma>' # LTS_\<epsilon>.remove_\<epsilon> (tl w))"
             using  VIII
-            using PDS.transition_rel.intros PDS_axioms append_self_conv2 op_labels.simps(1) r_into_rtranclp step_relp_def
+            using PDS.transition_rel.intros append_self_conv2 op_labels.simps(1) r_into_rtranclp step_relp_def
             by fastforce
           then have "(p2, LTS_\<epsilon>.remove_\<epsilon> (\<gamma>2' @ tl w)) \<Rightarrow>\<^sup>* (p, \<gamma>' # LTS_\<epsilon>.remove_\<epsilon> (tl w))"
             by (simp add: LTS_\<epsilon>.remove_\<epsilon>_append_dist \<gamma>2'_\<gamma>2)
@@ -1702,13 +1687,13 @@ next
           using VII by auto
         then show ?thesis
           using \<open>is_Ctr_Ext q\<close>
-          by (metis LTS_\<epsilon>.ffffffff ctr_loc.distinct_disc(1) w_tl_\<epsilon>)
+          by (metis LTS_\<epsilon>.ffffffff w_tl_\<epsilon>)
       qed
     next
       case (add_trans_push_1 p2 \<gamma>2 p1 \<gamma>1 \<gamma>'' q1')
       then have t_def: "t = (Ctr_Loc p1, Some \<gamma>1, Ctr_Loc_Ext p1 \<gamma>1)"
         using local.add_trans_pop(1) local.add_trans_pop p1_\<gamma>_p2_w2_q'_p(1) t_def by blast
-      have init_Ai: "\<nexists>q \<gamma> q'. (q, \<gamma>, Ctr_Loc q') \<in> Ai \<and> q' \<in> P_locs"
+      have init_Ai: "\<nexists>q \<gamma> q'. (q, \<gamma>, Ctr_Loc q') \<in> Ai"
         using step(1,2) step(4)
         using agagagagagaga'''''''''
         by (meson r_into_rtranclp)
@@ -1717,7 +1702,7 @@ next
         have "(ss, w) \<in> LTS.path_with_word Ai"
           using Suc(3) LTS.askdjfklasjflksa by metis
         moreover 
-        have "\<nexists>q \<gamma> q'. (q, \<gamma>, Ctr_Loc q') \<in> Ai \<and> q' \<in> P_locs"
+        have "\<nexists>q \<gamma> q'. (q, \<gamma>, Ctr_Loc q') \<in> Ai"
           using init_Ai by auto
         moreover 
         have "0 < count (transitions_of (ss, w)) t"
@@ -1726,9 +1711,8 @@ next
         have "t = (Ctr_Loc p1, Some \<gamma>1, Ctr_Loc_Ext p1 \<gamma>1)"
           using t_def by auto
         moreover 
-        have "p1 \<in> P_locs"
-          by (meson LTS.step_relp_def local.add_trans_push_1(2) step_relp'_P_locs2 transition_rel.intros)
-          
+        have "Ctr_Loc p1 \<in> P_locs"
+          using P_locs_def by fastforce
         ultimately
         show "hd (transition_list (ss, w)) = t \<and> count (transitions_of (ss, w)) t = 1"
           using xxxxxxxxxxxxxxx[of ss w Ai t] by auto
@@ -1779,7 +1763,7 @@ next
       note XIII = add_trans_push_2(2)
       have t_def: "t = (Ctr_Loc_Ext p1 \<gamma>1, Some \<gamma>'', q')"
         using local.add_trans_swap(1) local.add_trans_push_2 p1_\<gamma>_p2_w2_q'_p(1) t_def by blast
-      have init_Ai: "\<nexists>q \<gamma> q'. (q, \<gamma>, Ctr_Loc q') \<in> Ai \<and> q' \<in> P_locs"
+      have init_Ai: "\<nexists>q \<gamma> q'. (q, \<gamma>, Ctr_Loc q') \<in> Ai"
         using step(1,2) step(4)
         using agagagagagaga'''''''''
         by (meson r_into_rtranclp)
@@ -1799,11 +1783,11 @@ next
            ddd: "(q', v, v_ss, q) \<in> LTS.transition_star_states Ai"
         by auto
       from step(3)[of p u u_ss "Ctr_Loc_Ext p1 \<gamma>1"] X_1 have
-        "(is_Ctr_Loc (Ctr_Loc_Ext p1 \<gamma>1) \<longrightarrow>
+        "(\<not>is_Ctr_Ext (Ctr_Loc_Ext p1 \<gamma>1) \<longrightarrow>
            (\<exists>p' w'. (Ctr_Loc p', w', Ctr_Loc_Ext p1 \<gamma>1) \<in> LTS_\<epsilon>.transition_star_\<epsilon> A \<and> (p', w') \<Rightarrow>\<^sup>* (p, LTS_\<epsilon>.remove_\<epsilon> u))) \<and>
          (is_Ctr_Ext (Ctr_Loc_Ext p1 \<gamma>1) \<longrightarrow> 
            (the_Ext_Ctr_Loc (Ctr_Loc_Ext p1 \<gamma>1), [the_Ext_Label (Ctr_Loc_Ext p1 \<gamma>1)]) \<Rightarrow>\<^sup>* (p, LTS_\<epsilon>.remove_\<epsilon> u))"
-        using step.prems(1) step.prems(2) by blast
+        using step.prems(1) step.prems(2) by auto 
       then have "(the_Ext_Ctr_Loc (Ctr_Loc_Ext p1 \<gamma>1), [the_Ext_Label (Ctr_Loc_Ext p1 \<gamma>1)]) \<Rightarrow>\<^sup>* (p, LTS_\<epsilon>.remove_\<epsilon> u)"
         by auto
       then have "(p1, [\<gamma>1]) \<Rightarrow>\<^sup>* (p, LTS_\<epsilon>.remove_\<epsilon> u)"
@@ -1816,7 +1800,7 @@ next
       have "(q', v, v_ss, q) \<in> LTS.transition_star_states Ai"
         by (simp add: \<open>(q', v, v_ss, q) \<in> LTS.transition_star_states Ai\<close>)
       have inddd:
-        "(is_Ctr_Loc q \<longrightarrow> (\<exists>p' w'. (Ctr_Loc p', w', q) \<in> LTS_\<epsilon>.transition_star_\<epsilon> A \<and> (p', w') \<Rightarrow>\<^sup>* (p2, LTS_\<epsilon>.remove_\<epsilon> (\<gamma>2\<epsilon> @ v)))) \<and>
+        "(\<not>is_Ctr_Ext q \<longrightarrow> (\<exists>p' w'. (Ctr_Loc p', w', q) \<in> LTS_\<epsilon>.transition_star_\<epsilon> A \<and> (p', w') \<Rightarrow>\<^sup>* (p2, LTS_\<epsilon>.remove_\<epsilon> (\<gamma>2\<epsilon> @ v)))) \<and>
          (is_Ctr_Ext q \<longrightarrow> (the_Ext_Ctr_Loc q, [the_Ext_Label q]) \<Rightarrow>\<^sup>* (p2, LTS_\<epsilon>.remove_\<epsilon> (\<gamma>2\<epsilon> @ v)))"
       proof -
         have one: "length \<gamma>2ss = Suc (length \<gamma>2\<epsilon>)"
@@ -1890,16 +1874,16 @@ next
           
         from this Suc(1)[of p2 "\<gamma>2\<epsilon> @ v" "\<gamma>2ss @ tl v_ss" q]
         show
-          "(is_Ctr_Loc q \<longrightarrow> (\<exists>p' w'. (Ctr_Loc p', w', q) \<in> LTS_\<epsilon>.transition_star_\<epsilon> A \<and> (p', w') \<Rightarrow>\<^sup>* (p2, LTS_\<epsilon>.remove_\<epsilon> (\<gamma>2\<epsilon> @ v)))) \<and>
+          "(\<not>is_Ctr_Ext q \<longrightarrow> (\<exists>p' w'. (Ctr_Loc p', w', q) \<in> LTS_\<epsilon>.transition_star_\<epsilon> A \<and> (p', w') \<Rightarrow>\<^sup>* (p2, LTS_\<epsilon>.remove_\<epsilon> (\<gamma>2\<epsilon> @ v)))) \<and>
            (is_Ctr_Ext q \<longrightarrow> (the_Ext_Ctr_Loc q, [the_Ext_Label q]) \<Rightarrow>\<^sup>* (p2, LTS_\<epsilon>.remove_\<epsilon> (\<gamma>2\<epsilon> @ v)))"
           using \<open>j = count (transitions_of' (Ctr_Loc p2, \<gamma>2\<epsilon> @ v, \<gamma>2ss @ tl v_ss, q)) t\<close> by fastforce
       qed
 
       show ?thesis
-      proof (cases "is_Ctr_Loc q")
+      proof (cases "is_Ctr_Loc q \<or> is_State q")
         case True
         have "(\<exists>p' w'. (Ctr_Loc p', w', q) \<in> LTS_\<epsilon>.transition_star_\<epsilon> A \<and> (p', w') \<Rightarrow>\<^sup>* (p2, LTS_\<epsilon>.remove_\<epsilon> (\<gamma>2\<epsilon> @ v)))"
-          using True \<open>(is_Ctr_Loc q \<longrightarrow> (\<exists>p' w'. (Ctr_Loc p', w', q) \<in> LTS_\<epsilon>.transition_star_\<epsilon> A \<and> (p', w') \<Rightarrow>\<^sup>* (p2, LTS_\<epsilon>.remove_\<epsilon> (\<gamma>2\<epsilon> @ v)))) \<and> (is_Ctr_Ext q \<longrightarrow> (the_Ext_Ctr_Loc q, [the_Ext_Label q]) \<Rightarrow>\<^sup>* (p2, LTS_\<epsilon>.remove_\<epsilon> (\<gamma>2\<epsilon> @ v)))\<close> by fastforce
+          using True \<open>(\<not>is_Ctr_Ext q \<longrightarrow> (\<exists>p' w'. (Ctr_Loc p', w', q) \<in> LTS_\<epsilon>.transition_star_\<epsilon> A \<and> (p', w') \<Rightarrow>\<^sup>* (p2, LTS_\<epsilon>.remove_\<epsilon> (\<gamma>2\<epsilon> @ v)))) \<and> (is_Ctr_Ext q \<longrightarrow> (the_Ext_Ctr_Loc q, [the_Ext_Label q]) \<Rightarrow>\<^sup>* (p2, LTS_\<epsilon>.remove_\<epsilon> (\<gamma>2\<epsilon> @ v)))\<close> by fastforce
         then obtain p' w' where "(Ctr_Loc p', w', q) \<in> LTS_\<epsilon>.transition_star_\<epsilon> A \<and> (p', w') \<Rightarrow>\<^sup>* (p2, LTS_\<epsilon>.remove_\<epsilon> (\<gamma>2\<epsilon> @ v))"
           by auto
         then have "(p', w') \<Rightarrow>\<^sup>* (p2, LTS_\<epsilon>.remove_\<epsilon> (\<gamma>2\<epsilon> @ v))"
@@ -1911,7 +1895,7 @@ next
             by (metis LTS_\<epsilon>.\<epsilon>_exp_def LTS_\<epsilon>.remove_\<epsilon>_append_dist LTS_\<epsilon>.remove_\<epsilon>_def append_Cons self_append_conv2) 
           moreover
           from XIII have "(p2, \<gamma>2 #(LTS_\<epsilon>.remove_\<epsilon> v)) \<Rightarrow>\<^sup>* (p1, \<gamma>1#\<gamma>''#LTS_\<epsilon>.remove_\<epsilon> v)"
-            by (metis PDS.transition_rel.intros PDS_axioms append_Cons append_Nil op_labels.simps(3) r_into_rtranclp step_relp_def)
+            by (metis PDS.transition_rel.intros append_Cons append_Nil op_labels.simps(3) r_into_rtranclp step_relp_def)
           ultimately
           show "(p2, LTS_\<epsilon>.remove_\<epsilon> (\<gamma>2\<epsilon> @ v)) \<Rightarrow>\<^sup>* (p1, \<gamma>1#\<gamma>''#LTS_\<epsilon>.remove_\<epsilon> v)"
             by auto
@@ -1926,7 +1910,8 @@ next
       next
         case False
         then have "(the_Ext_Ctr_Loc q, [the_Ext_Label q]) \<Rightarrow>\<^sup>* (p2, LTS_\<epsilon>.remove_\<epsilon> (\<gamma>2\<epsilon> @ v))"
-          using inddd ctr_loc.exhaust_disc by blast 
+          using inddd state.exhaust_disc
+          by blast
         have "(p2, LTS_\<epsilon>.remove_\<epsilon> (\<gamma>2\<epsilon> @ v))  \<Rightarrow>\<^sup>* (p1, \<gamma>1 # \<gamma>'' # LTS_\<epsilon>.remove_\<epsilon> v)"
           by (metis (mono_tags, hide_lams) LTS_\<epsilon>.\<epsilon>_exp_def LTS_\<epsilon>.remove_\<epsilon>_append_dist LTS_\<epsilon>.remove_\<epsilon>_def XIII XI_1 append_Cons append_Nil op_labels.simps(3) r_into_rtranclp step_relp_def2)
           
@@ -1937,51 +1922,78 @@ next
           by (metis LTS_\<epsilon>.ffffffff LTS_\<epsilon>.remove_\<epsilon>_append_dist append_Cons append_Nil bbb hd_Cons_tl list.distinct(1) list.inject)
           
         show ?thesis
-          using False \<open>(p, LTS_\<epsilon>.remove_\<epsilon> u @ \<gamma>'' # LTS_\<epsilon>.remove_\<epsilon> v) = (p, LTS_\<epsilon>.remove_\<epsilon> w)\<close> \<open>(p1, \<gamma>1 # \<gamma>'' # LTS_\<epsilon>.remove_\<epsilon> v) \<Rightarrow>\<^sup>* (p, LTS_\<epsilon>.remove_\<epsilon> u @ \<gamma>'' # LTS_\<epsilon>.remove_\<epsilon> v)\<close> \<open>(p2, LTS_\<epsilon>.remove_\<epsilon> (\<gamma>2\<epsilon> @ v)) \<Rightarrow>\<^sup>* (p1, \<gamma>1 # \<gamma>'' # LTS_\<epsilon>.remove_\<epsilon> v)\<close> \<open>(the_Ext_Ctr_Loc q, [the_Ext_Label q]) \<Rightarrow>\<^sup>* (p2, LTS_\<epsilon>.remove_\<epsilon> (\<gamma>2\<epsilon> @ v))\<close> by fastforce
+          using False \<open>(p, LTS_\<epsilon>.remove_\<epsilon> u @ \<gamma>'' # LTS_\<epsilon>.remove_\<epsilon> v) = (p, LTS_\<epsilon>.remove_\<epsilon> w)\<close> \<open>(p1, \<gamma>1 # \<gamma>'' # LTS_\<epsilon>.remove_\<epsilon> v) \<Rightarrow>\<^sup>* (p, LTS_\<epsilon>.remove_\<epsilon> u @ \<gamma>'' # LTS_\<epsilon>.remove_\<epsilon> v)\<close> \<open>(p2, LTS_\<epsilon>.remove_\<epsilon> (\<gamma>2\<epsilon> @ v)) \<Rightarrow>\<^sup>* (p1, \<gamma>1 # \<gamma>'' # LTS_\<epsilon>.remove_\<epsilon> v)\<close> \<open>(the_Ext_Ctr_Loc q, [the_Ext_Label q]) \<Rightarrow>\<^sup>* (p2, LTS_\<epsilon>.remove_\<epsilon> (\<gamma>2\<epsilon> @ v))\<close>
+          by (metis (no_types, lifting) inddd rtranclp_trans) 
+
       qed
     qed
   qed
 qed
 
-term accepts_\<epsilon>
-term language_\<epsilon>
-thm theorem_3_2
-
-
-
-fun make_normal where
-  "make_normal (p, w) = (the_Ctr_Loc p, w)"
+lemma lemma_3_4'':
+  assumes "post_star_rules\<^sup>*\<^sup>* A A'"
+  assumes "\<nexists>q \<gamma> q'. (q, \<gamma>, Ctr_Loc q') \<in> A"
+  assumes "\<forall>a b c. (a, b, c) \<in> A \<longrightarrow> a \<notin> New_Aut_states \<and> c \<notin> New_Aut_states"
+  assumes "(Ctr_Loc p, w, q) \<in> LTS.transition_star A'"
+  shows "(\<not>is_Ctr_Ext q \<longrightarrow> (\<exists>p' w'. (Ctr_Loc p', w', q) \<in> LTS_\<epsilon>.transition_star_\<epsilon> A \<and> (p',w') \<Rightarrow>\<^sup>* (p, LTS_\<epsilon>.remove_\<epsilon> w))) \<and>
+         (is_Ctr_Ext q \<longrightarrow> (the_Ext_Ctr_Loc q, [the_Ext_Label q]) \<Rightarrow>\<^sup>* (p, LTS_\<epsilon>.remove_\<epsilon> w))"
+  using lemma_3_4' assms by (metis LTS.transition_star_transition_star_states) 
 
 lemma lemma_3_4:
-  assumes "post_star_rules\<^sup>*\<^sup>* A A'"
-  assumes "\<nexists>q \<gamma> q'. (q, \<gamma>, Ctr_Loc q') \<in> A \<and> q' \<in> P_locs"
-  assumes "\<forall>a b c. (a, b, c) \<in> A \<longrightarrow> is_Ctr_Loc a \<and> is_Ctr_Loc c"
-  shows "make_normal ` {c. accepts_\<epsilon> A' c} = post_star (make_normal `(language_\<epsilon> A))"
-proof (rule; rule)
-  fix c :: "'ctr_loc \<times> 'label list"
-  define p where "p = fst c"
-  define w where "w = snd c"
-  assume "c \<in> make_normal ` {c. accepts_\<epsilon> A' c}"
-  show "c \<in> post_star (make_normal ` language_\<epsilon> A)"
-    sorry
-next
-  fix c :: "'ctr_loc \<times> 'label list"
-  define p where "p = fst c"
-  define w where "w = snd c"
-  assume "c \<in> post_star (make_normal ` language_\<epsilon> A)"
-  then obtain p' w' where "(p', w') \<Rightarrow>\<^sup>* (p, w) \<and> (p', w') \<in> make_normal ` language_\<epsilon> A"
-    by (smt (verit, ccfv_SIG) LTS.post_star_def mem_Collect_eq p_def prod.collapse w_def)
-  then have "(Ctr_Loc p', w') \<in> language_\<epsilon> A"
-  
-  show "c \<in> make_normal ` {c. accepts_\<epsilon> A' c}"
-    sorry
-qed
+  assumes "saturation post_star_rules A A'"
+  assumes "\<nexists>q \<gamma> q'. (q, \<gamma>, Ctr_Loc q') \<in> A"
+  assumes "\<forall>a b c. (a, b, c) \<in> A \<longrightarrow> a \<notin> New_Aut_states \<and> c \<notin> New_Aut_states"
+  assumes "(Ctr_Loc p, w, q) \<in> LTS.transition_star A'"
+  shows "(\<not>is_Ctr_Ext q \<longrightarrow> (\<exists>p' w'. (Ctr_Loc p', w', q) \<in> LTS_\<epsilon>.transition_star_\<epsilon> A \<and> (p',w') \<Rightarrow>\<^sup>* (p, LTS_\<epsilon>.remove_\<epsilon> w))) \<and>
+         (is_Ctr_Ext q \<longrightarrow> (the_Ext_Ctr_Loc q, [the_Ext_Label q]) \<Rightarrow>\<^sup>* (p, LTS_\<epsilon>.remove_\<epsilon> w))"
+  using lemma_3_4'' assms saturation_def by metis 
 
-(*   (('ctr_loc, 'label) ctr_loc \<times> 'label list) set   *)
-  term post_star
 
 theorem theorem_3_3:
-  assumes "post_star_rules\<^sup>*\<^sup>* A A'"
+  assumes "saturation post_star_rules A A'"
+  assumes "\<nexists>q \<gamma> q'. (q, \<gamma>, Ctr_Loc q') \<in> A"
+  assumes "\<forall>a b c. (a, b, c) \<in> A \<longrightarrow> a \<notin> New_Aut_states \<and> c \<notin> New_Aut_states"
+  shows "{c. accepts_\<epsilon> A' c} = post_star (language_\<epsilon> A)"
+proof (rule; rule)
+  fix c :: "('ctr_loc, 'label) conf"
+  define p where "p = fst c"
+  define w where "w = snd c"
+  assume "c \<in> post_star (language_\<epsilon> A)"
+  then obtain p' w' where "(p', w') \<Rightarrow>\<^sup>* (p, w) \<and> (p', w') \<in> language_\<epsilon> A"
+    by (smt (verit, ccfv_SIG) LTS.post_star_def mem_Collect_eq p_def prod.collapse w_def)
+  then have "accepts_\<epsilon> A' (p, w)"
+    using lemma_3_3[of p' w' p w A A'] assms(1) by auto 
+  then have "accepts_\<epsilon> A' c"
+    unfolding p_def w_def by auto
+  then show "c \<in> {c. accepts_\<epsilon> A' c}"
+    by auto
+next
+  fix c :: "('ctr_loc, 'label) conf"
+  define p where "p = fst c"
+  define w where "w = snd c"
+  assume "c \<in>  {c. accepts_\<epsilon> A' c}"
+  then have "accepts_\<epsilon> A' (p,w)"
+    unfolding p_def w_def by auto
+  then obtain q where q_p: "q\<in>F_locs" "(Ctr_Loc p, w, q) \<in> LTS_\<epsilon>.transition_star_\<epsilon> A'" 
+    unfolding accepts_\<epsilon>_def by auto
+  then obtain w' where w'_def: "LTS_\<epsilon>.\<epsilon>_exp w' w \<and> (Ctr_Loc p, w', q) \<in> LTS.transition_star A'"
+    by (meson LTS_\<epsilon>.epsilon_lemma3)
+  then have ttt: "(Ctr_Loc p, w', q) \<in> LTS.transition_star A'"
+    by auto
+  have "\<not> is_Ctr_Ext q"
+    using q_p(2) sorry
+  then obtain p' w'a where "(Ctr_Loc p', w'a, q) \<in> LTS_\<epsilon>.transition_star_\<epsilon> A \<and> (p', w'a) \<Rightarrow>\<^sup>* (p, LTS_\<epsilon>.remove_\<epsilon> w')"
+    using lemma_3_4[OF assms(1) assms(2) assms(3) ttt] by auto
+  then have "(Ctr_Loc p', w'a, q) \<in> LTS_\<epsilon>.transition_star_\<epsilon> A \<and> (p', w'a) \<Rightarrow>\<^sup>* (p, w)"
+    using w'_def by (metis LTS_\<epsilon>.\<epsilon>_exp_def LTS_\<epsilon>.remove_\<epsilon>_def \<open>LTS_\<epsilon>.\<epsilon>_exp w' w \<and> (Ctr_Loc p, w', q) \<in> LTS.transition_star A'\<close>)
+  then have "(p,w) \<in> post_star (language_\<epsilon> A)"
+    using \<open>q \<in> F_locs\<close> unfolding LTS.post_star_def accepts_\<epsilon>_def language_\<epsilon>_def by fastforce
+  then show "c \<in> post_star (language_\<epsilon> A)"
+    unfolding p_def w_def by auto
+qed
+
+
+
 
 
 
